QCP_examples/humaneval/spec_logic_rewrite_c_files/C_7_goal.v
@@ -1,0 +1,1011 @@
+Require Import Coq.ZArith.ZArith.
+Require Import Coq.Bool.Bool.
+Require Import Coq.Strings.String.
+Require Import Coq.Strings.Ascii.
+Require Import Coq.Lists.List.
+Require Import Coq.Classes.RelationClasses.
+Require Import Coq.Classes.Morphisms.
+Require Import Coq.micromega.Psatz.
+Require Import Coq.Sorting.Permutation.
+From AUXLib Require Import int_auto Axioms Feq Idents ListLib VMap.
+Require Import SetsClass.SetsClass. Import SetsNotation.
+From SimpleC.SL Require Import Mem SeparationLogic.
+Require Import Logic.LogicGenerator.demo932.Interface.
+Local Open Scope Z_scope.
+Local Open Scope sets.
+Local Open Scope string_scope.
+Local Open Scope list.
+Import naive_C_Rules.
+Require Import SimpleC.StdLib.string_lib.
+Require Import SimpleC.EE.coins_7.
+Local Open Scope sac.
+From SimpleC.EE.QCP_demos_LLM Require Import ptr_array2_strategy_goal.
+From SimpleC.EE.QCP_demos_LLM Require Import ptr_array2_strategy_proof.
+From SimpleC.EE.QCP_demos_LLM Require Import char_array_strategy_goal.
+From SimpleC.EE.QCP_demos_LLM Require Import char_array_strategy_proof.
+From SimpleC.StdLib Require Import string_strategy_goal.
+From SimpleC.StdLib Require Import string_strategy_proof.
+
+(*----- Function filter_by_substring -----*)
+
+Definition filter_by_substring_safety_wit_1 := 
+forall (substring_pre: Z) (strings_size_pre: Z) (strings_pre: Z) (substring_addr: Z) (strings_addr: Z) (substring_l: (@list Z)) (rows: (@list (@list Z))) (retval: Z) (PreH1 : (retval <> 0)) (PreH2 : (0 <= ((string_length (substring_l)) + 1 ))) (PreH3 : (strings_pre = strings_addr)) (PreH4 : (substring_pre = substring_addr)) (PreH5 : (0 <= strings_size_pre)) (PreH6 : (strings_size_pre <= 100)) (PreH7 : (rows_well_formed_7 rows strings_size_pre )) (PreH8 : (problem_7_pre_z rows )) (PreH9 : (valid_string substring_l )) (PreH10 : ((string_length (substring_l)) < INT_MAX)) ,
+  ((&((retval)  # "<anonymous struct>" ->ₛ "data")) # Ptr  |->_)
+  **  ((&((retval)  # "<anonymous struct>" ->ₛ "size")) # Int  |->_)
+  **  (CharArray.full substring_pre ((string_length (substring_l)) + 1 ) (c_string (substring_l)) )
+  **  ((( &( "out" ) )) # Ptr  |-> retval)
+  **  ((( &( "substring" ) )) # Ptr  |-> substring_pre)
+  **  ((( &( "strings_size" ) )) # Int  |-> strings_size_pre)
+  **  ((( &( "strings" ) )) # Ptr  |-> strings_pre)
+  **  (CharPtrArray2.full strings_pre strings_size_pre rows )
+|--
+  “ (0 <= INT_MAX) ” 
+  &&  “ ((INT_MIN) <= 0) ”
+.
+
+Definition filter_by_substring_safety_wit_2 := 
+forall (substring_pre: Z) (strings_size_pre: Z) (strings_pre: Z) (substring_addr: Z) (strings_addr: Z) (substring_l: (@list Z)) (rows: (@list (@list Z))) (retval: Z) (retval_2: Z) (PreH1 : (retval_2 <> 0)) (PreH2 : (retval <> 0)) (PreH3 : (0 <= ((string_length (substring_l)) + 1 ))) (PreH4 : (strings_pre = strings_addr)) (PreH5 : (substring_pre = substring_addr)) (PreH6 : (0 <= strings_size_pre)) (PreH7 : (strings_size_pre <= 100)) (PreH8 : (rows_well_formed_7 rows strings_size_pre )) (PreH9 : (problem_7_pre_z rows )) (PreH10 : (valid_string substring_l )) (PreH11 : ((string_length (substring_l)) < INT_MAX)) ,
+  ((( &( "output_size" ) )) # Int  |->_)
+  **  ((( &( "data" ) )) # Ptr  |-> retval_2)
+  **  (PtrArray.undef_seg retval_2 0 strings_size_pre )
+  **  ((&((retval)  # "<anonymous struct>" ->ₛ "data")) # Ptr  |-> retval_2)
+  **  ((&((retval)  # "<anonymous struct>" ->ₛ "size")) # Int  |-> 0)
+  **  (CharArray.full substring_pre ((string_length (substring_l)) + 1 ) (c_string (substring_l)) )
+  **  ((( &( "out" ) )) # Ptr  |-> retval)
+  **  ((( &( "substring" ) )) # Ptr  |-> substring_pre)
+  **  ((( &( "strings_size" ) )) # Int  |-> strings_size_pre)
+  **  ((( &( "strings" ) )) # Ptr  |-> strings_pre)
+  **  (CharPtrArray2.full strings_pre strings_size_pre rows )
+|--
+  “ (0 <= INT_MAX) ” 
+  &&  “ ((INT_MIN) <= 0) ”
+.
+
+Definition filter_by_substring_safety_wit_3 := 
+forall (substring_pre: Z) (strings_size_pre: Z) (strings_pre: Z) (substring_addr: Z) (strings_addr: Z) (substring_l: (@list Z)) (rows: (@list (@list Z))) (retval: Z) (retval_2: Z) (PreH1 : (retval_2 <> 0)) (PreH2 : (retval <> 0)) (PreH3 : (0 <= ((string_length (substring_l)) + 1 ))) (PreH4 : (strings_pre = strings_addr)) (PreH5 : (substring_pre = substring_addr)) (PreH6 : (0 <= strings_size_pre)) (PreH7 : (strings_size_pre <= 100)) (PreH8 : (rows_well_formed_7 rows strings_size_pre )) (PreH9 : (problem_7_pre_z rows )) (PreH10 : (valid_string substring_l )) (PreH11 : ((string_length (substring_l)) < INT_MAX)) ,
+  ((( &( "cur" ) )) # Ptr  |->_)
+  **  ((( &( "output_size" ) )) # Int  |-> 0)
+  **  ((( &( "data" ) )) # Ptr  |-> retval_2)
+  **  (PtrArray.undef_seg retval_2 0 strings_size_pre )
+  **  ((&((retval)  # "<anonymous struct>" ->ₛ "data")) # Ptr  |-> retval_2)
+  **  ((&((retval)  # "<anonymous struct>" ->ₛ "size")) # Int  |-> 0)
+  **  (CharArray.full substring_pre ((string_length (substring_l)) + 1 ) (c_string (substring_l)) )
+  **  ((( &( "out" ) )) # Ptr  |-> retval)
+  **  ((( &( "substring" ) )) # Ptr  |-> substring_pre)
+  **  ((( &( "strings_size" ) )) # Int  |-> strings_size_pre)
+  **  ((( &( "strings" ) )) # Ptr  |-> strings_pre)
+  **  (CharPtrArray2.full strings_pre strings_size_pre rows )
+|--
+  “ (0 <= INT_MAX) ” 
+  &&  “ ((INT_MIN) <= 0) ”
+.
+
+Definition filter_by_substring_safety_wit_4 := 
+forall (substring_pre: Z) (strings_size_pre: Z) (strings_pre: Z) (substring_addr: Z) (strings_addr: Z) (substring_l: (@list Z)) (rows: (@list (@list Z))) (retval: Z) (retval_2: Z) (PreH1 : (retval_2 <> 0)) (PreH2 : (retval <> 0)) (PreH3 : (0 <= ((string_length (substring_l)) + 1 ))) (PreH4 : (strings_pre = strings_addr)) (PreH5 : (substring_pre = substring_addr)) (PreH6 : (0 <= strings_size_pre)) (PreH7 : (strings_size_pre <= 100)) (PreH8 : (rows_well_formed_7 rows strings_size_pre )) (PreH9 : (problem_7_pre_z rows )) (PreH10 : (valid_string substring_l )) (PreH11 : ((string_length (substring_l)) < INT_MAX)) ,
+  ((( &( "hit" ) )) # Ptr  |->_)
+  **  ((( &( "cur" ) )) # Ptr  |-> 0)
+  **  ((( &( "output_size" ) )) # Int  |-> 0)
+  **  ((( &( "data" ) )) # Ptr  |-> retval_2)
+  **  (PtrArray.undef_seg retval_2 0 strings_size_pre )
+  **  ((&((retval)  # "<anonymous struct>" ->ₛ "data")) # Ptr  |-> retval_2)
+  **  ((&((retval)  # "<anonymous struct>" ->ₛ "size")) # Int  |-> 0)
+  **  (CharArray.full substring_pre ((string_length (substring_l)) + 1 ) (c_string (substring_l)) )
+  **  ((( &( "out" ) )) # Ptr  |-> retval)
+  **  ((( &( "substring" ) )) # Ptr  |-> substring_pre)
+  **  ((( &( "strings_size" ) )) # Int  |-> strings_size_pre)
+  **  ((( &( "strings" ) )) # Ptr  |-> strings_pre)
+  **  (CharPtrArray2.full strings_pre strings_size_pre rows )
+|--
+  “ (0 <= INT_MAX) ” 
+  &&  “ ((INT_MIN) <= 0) ”
+.
+
+Definition filter_by_substring_safety_wit_5 := 
+forall (substring_pre: Z) (strings_size_pre: Z) (strings_pre: Z) (substring_addr: Z) (strings_addr: Z) (substring_l: (@list Z)) (rows: (@list (@list Z))) (retval: Z) (retval_2: Z) (PreH1 : (retval_2 <> 0)) (PreH2 : (retval <> 0)) (PreH3 : (0 <= ((string_length (substring_l)) + 1 ))) (PreH4 : (strings_pre = strings_addr)) (PreH5 : (substring_pre = substring_addr)) (PreH6 : (0 <= strings_size_pre)) (PreH7 : (strings_size_pre <= 100)) (PreH8 : (rows_well_formed_7 rows strings_size_pre )) (PreH9 : (problem_7_pre_z rows )) (PreH10 : (valid_string substring_l )) (PreH11 : ((string_length (substring_l)) < INT_MAX)) ,
+  ((( &( "i" ) )) # Int  |->_)
+  **  ((( &( "hit" ) )) # Ptr  |-> 0)
+  **  ((( &( "cur" ) )) # Ptr  |-> 0)
+  **  ((( &( "output_size" ) )) # Int  |-> 0)
+  **  ((( &( "data" ) )) # Ptr  |-> retval_2)
+  **  (PtrArray.undef_seg retval_2 0 strings_size_pre )
+  **  ((&((retval)  # "<anonymous struct>" ->ₛ "data")) # Ptr  |-> retval_2)
+  **  ((&((retval)  # "<anonymous struct>" ->ₛ "size")) # Int  |-> 0)
+  **  (CharArray.full substring_pre ((string_length (substring_l)) + 1 ) (c_string (substring_l)) )
+  **  ((( &( "out" ) )) # Ptr  |-> retval)
+  **  ((( &( "substring" ) )) # Ptr  |-> substring_pre)
+  **  ((( &( "strings_size" ) )) # Int  |-> strings_size_pre)
+  **  ((( &( "strings" ) )) # Ptr  |-> strings_pre)
+  **  (CharPtrArray2.full strings_pre strings_size_pre rows )
+|--
+  “ (0 <= INT_MAX) ” 
+  &&  “ ((INT_MIN) <= 0) ”
+.
+
+Definition filter_by_substring_safety_wit_6 := 
+forall (strings_size_pre: Z) (substring_addr: Z) (strings_addr: Z) (substring_l: (@list Z)) (rows: (@list (@list Z))) (row_ptr: Z) (output_rows: (@list (@list Z))) (output_ptrs: (@list Z)) (i: Z) (output_size: Z) (out: Z) (data: Z) (retval: Z) (PreH1 : (strstr_result (row_payload_z_7 ((Znth (i) (rows) ((@nil Z))))) substring_l retval row_ptr )) (PreH2 : (0 <= ((string_length (substring_l)) + 1 ))) (PreH3 : (0 <= ((string_length ((row_payload_z_7 ((Znth (i) (rows) ((@nil Z))))))) + 1 ))) (PreH4 : (0 <= i)) (PreH5 : (i < strings_size_pre)) (PreH6 : (0 <= output_size)) (PreH7 : (output_size <= i)) (PreH8 : (output_size = (Zlength (output_rows)))) (PreH9 : (output_size = (Zlength (output_ptrs)))) (PreH10 : (out <> 0)) (PreH11 : (data <> 0)) (PreH12 : (rows_well_formed_7 rows strings_size_pre )) (PreH13 : (row_well_formed_7 (Znth (i) (rows) ((@nil Z))) )) (PreH14 : (problem_7_pre_z rows )) (PreH15 : (valid_string substring_l )) (PreH16 : ((string_length (substring_l)) < INT_MAX)) (PreH17 : (filter_substring_state_7 rows substring_l i output_rows )) ,
+  (store_string row_ptr (row_payload_z_7 ((Znth (i) (rows) ((@nil Z))))) )
+  **  (store_string substring_addr substring_l )
+  **  ((( &( "i" ) )) # Int  |-> i)
+  **  ((( &( "output_size" ) )) # Int  |-> output_size)
+  **  ((( &( "strings" ) )) # Ptr  |-> strings_addr)
+  **  ((( &( "substring" ) )) # Ptr  |-> substring_addr)
+  **  ((( &( "strings_size" ) )) # Int  |-> strings_size_pre)
+  **  ((( &( "out" ) )) # Ptr  |-> out)
+  **  ((( &( "data" ) )) # Ptr  |-> data)
+  **  ((( &( "cur" ) )) # Ptr  |-> row_ptr)
+  **  ((( &( "hit" ) )) # Ptr  |-> retval)
+  **  ((&((out)  # "<anonymous struct>" ->ₛ "data")) # Ptr  |-> data)
+  **  ((&((out)  # "<anonymous struct>" ->ₛ "size")) # Int  |-> 0)
+  **  (CharPtrArray2.missing_i strings_addr strings_size_pre i row_ptr rows )
+  **  (((strings_addr + (i * sizeof(PTR) ) )) # Ptr  |-> row_ptr)
+  **  (PtrArray.seg data 0 output_size output_ptrs )
+  **  (PtrArray.undef_seg data output_size strings_size_pre )
+|--
+  “ (0 <= INT_MAX) ” 
+  &&  “ ((INT_MIN) <= 0) ”
+.
+
+Definition filter_by_substring_safety_wit_7 := 
+forall (strings_size_pre: Z) (substring_addr: Z) (strings_addr: Z) (substring_l: (@list Z)) (rows: (@list (@list Z))) (row_ptr: Z) (output_rows: (@list (@list Z))) (output_ptrs: (@list Z)) (i: Z) (output_size: Z) (hit: Z) (out: Z) (data: Z) (PreH1 : (0 <= ((string_length (substring_l)) + 1 ))) (PreH2 : (0 <= ((string_length ((row_payload_z_7 ((Znth (i) (rows) ((@nil Z))))))) + 1 ))) (PreH3 : (0 <= i)) (PreH4 : (i < strings_size_pre)) (PreH5 : (0 <= output_size)) (PreH6 : (output_size <= i)) (PreH7 : (output_size = (Zlength (output_rows)))) (PreH8 : (output_size = (Zlength (output_ptrs)))) (PreH9 : (hit <> 0)) (PreH10 : (out <> 0)) (PreH11 : (data <> 0)) (PreH12 : (rows_well_formed_7 rows strings_size_pre )) (PreH13 : (problem_7_pre_z rows )) (PreH14 : (valid_string substring_l )) (PreH15 : ((string_length (substring_l)) < INT_MAX)) (PreH16 : (filter_substring_state_7 rows substring_l i output_rows )) (PreH17 : (substring_hit_z_7 (row_payload_z_7 ((Znth (i) (rows) ((@nil Z))))) substring_l )) ,
+  (PtrArray.seg data 0 (output_size + 1 ) (app (output_ptrs) ((cons (row_ptr) ((@nil Z))))) )
+  **  (PtrArray.undef_seg data (output_size + 1 ) strings_size_pre )
+  **  (CharArray.full substring_addr ((string_length (substring_l)) + 1 ) (c_string (substring_l)) )
+  **  (CharArray.full row_ptr ((string_length ((row_payload_z_7 ((Znth (i) (rows) ((@nil Z))))))) + 1 ) (c_string ((row_payload_z_7 ((Znth (i) (rows) ((@nil Z))))))) )
+  **  ((( &( "i" ) )) # Int  |-> i)
+  **  ((( &( "output_size" ) )) # Int  |-> output_size)
+  **  ((( &( "strings" ) )) # Ptr  |-> strings_addr)
+  **  ((( &( "substring" ) )) # Ptr  |-> substring_addr)
+  **  ((( &( "strings_size" ) )) # Int  |-> strings_size_pre)
+  **  ((( &( "cur" ) )) # Ptr  |-> row_ptr)
+  **  ((( &( "hit" ) )) # Ptr  |-> hit)
+  **  ((( &( "out" ) )) # Ptr  |-> out)
+  **  ((( &( "data" ) )) # Ptr  |-> data)
+  **  ((&((out)  # "<anonymous struct>" ->ₛ "data")) # Ptr  |-> data)
+  **  ((&((out)  # "<anonymous struct>" ->ₛ "size")) # Int  |-> 0)
+  **  (CharPtrArray2.missing_i strings_addr strings_size_pre i row_ptr rows )
+  **  (((strings_addr + (i * sizeof(PTR) ) )) # Ptr  |-> row_ptr)
+|--
+  “ ((output_size + 1 ) <= INT_MAX) ” 
+  &&  “ ((INT_MIN) <= (output_size + 1 )) ”
+.
+
+Definition filter_by_substring_safety_wit_8 := 
+forall (strings_size_pre: Z) (substring_addr: Z) (strings_addr: Z) (substring_l: (@list Z)) (rows: (@list (@list Z))) (row_ptr: Z) (output_rows: (@list (@list Z))) (output_ptrs: (@list Z)) (i: Z) (output_size: Z) (hit: Z) (out: Z) (data: Z) (PreH1 : (0 <= ((string_length (substring_l)) + 1 ))) (PreH2 : (0 <= ((string_length ((row_payload_z_7 ((Znth (i) (rows) ((@nil Z))))))) + 1 ))) (PreH3 : (0 <= i)) (PreH4 : (i < strings_size_pre)) (PreH5 : (0 <= output_size)) (PreH6 : (output_size <= i)) (PreH7 : (output_size = (Zlength (output_rows)))) (PreH8 : (output_size = (Zlength (output_ptrs)))) (PreH9 : (hit <> 0)) (PreH10 : (out <> 0)) (PreH11 : (data <> 0)) (PreH12 : (rows_well_formed_7 rows strings_size_pre )) (PreH13 : (problem_7_pre_z rows )) (PreH14 : (valid_string substring_l )) (PreH15 : ((string_length (substring_l)) < INT_MAX)) (PreH16 : (filter_substring_state_7 rows substring_l i output_rows )) (PreH17 : (substring_hit_z_7 (row_payload_z_7 ((Znth (i) (rows) ((@nil Z))))) substring_l )) ,
+  (PtrArray.seg data 0 (output_size + 1 ) (app (output_ptrs) ((cons (row_ptr) ((@nil Z))))) )
+  **  (PtrArray.undef_seg data (output_size + 1 ) strings_size_pre )
+  **  (CharArray.full substring_addr ((string_length (substring_l)) + 1 ) (c_string (substring_l)) )
+  **  (CharArray.full row_ptr ((string_length ((row_payload_z_7 ((Znth (i) (rows) ((@nil Z))))))) + 1 ) (c_string ((row_payload_z_7 ((Znth (i) (rows) ((@nil Z))))))) )
+  **  ((( &( "i" ) )) # Int  |-> i)
+  **  ((( &( "output_size" ) )) # Int  |-> output_size)
+  **  ((( &( "strings" ) )) # Ptr  |-> strings_addr)
+  **  ((( &( "substring" ) )) # Ptr  |-> substring_addr)
+  **  ((( &( "strings_size" ) )) # Int  |-> strings_size_pre)
+  **  ((( &( "cur" ) )) # Ptr  |-> row_ptr)
+  **  ((( &( "hit" ) )) # Ptr  |-> hit)
+  **  ((( &( "out" ) )) # Ptr  |-> out)
+  **  ((( &( "data" ) )) # Ptr  |-> data)
+  **  ((&((out)  # "<anonymous struct>" ->ₛ "data")) # Ptr  |-> data)
+  **  ((&((out)  # "<anonymous struct>" ->ₛ "size")) # Int  |-> 0)
+  **  (CharPtrArray2.missing_i strings_addr strings_size_pre i row_ptr rows )
+  **  (((strings_addr + (i * sizeof(PTR) ) )) # Ptr  |-> row_ptr)
+|--
+  “ (1 <= INT_MAX) ” 
+  &&  “ ((INT_MIN) <= 1) ”
+.
+
+Definition filter_by_substring_safety_wit_9 := 
+forall (strings_size_pre: Z) (substring_addr: Z) (strings_addr: Z) (substring_l: (@list Z)) (rows: (@list (@list Z))) (output_rows: (@list (@list Z))) (output_ptrs: (@list Z)) (i: Z) (output_size: Z) (out: Z) (data: Z) (cur: Z) (hit: Z) (PreH1 : (0 <= i)) (PreH2 : (i < strings_size_pre)) (PreH3 : (0 <= output_size)) (PreH4 : (output_size <= (i + 1 ))) (PreH5 : (output_size = (Zlength (output_rows)))) (PreH6 : (output_size = (Zlength (output_ptrs)))) (PreH7 : (out <> 0)) (PreH8 : (data <> 0)) (PreH9 : (rows_well_formed_7 rows strings_size_pre )) (PreH10 : (problem_7_pre_z rows )) (PreH11 : (valid_string substring_l )) (PreH12 : ((string_length (substring_l)) < INT_MAX)) (PreH13 : (filter_substring_state_7 rows substring_l (i + 1 ) output_rows )) ,
+  ((( &( "i" ) )) # Int  |-> i)
+  **  ((( &( "output_size" ) )) # Int  |-> output_size)
+  **  ((( &( "strings" ) )) # Ptr  |-> strings_addr)
+  **  ((( &( "substring" ) )) # Ptr  |-> substring_addr)
+  **  ((( &( "strings_size" ) )) # Int  |-> strings_size_pre)
+  **  ((( &( "out" ) )) # Ptr  |-> out)
+  **  ((( &( "data" ) )) # Ptr  |-> data)
+  **  ((( &( "cur" ) )) # Ptr  |-> cur)
+  **  ((( &( "hit" ) )) # Ptr  |-> hit)
+  **  ((&((out)  # "<anonymous struct>" ->ₛ "data")) # Ptr  |-> data)
+  **  ((&((out)  # "<anonymous struct>" ->ₛ "size")) # Int  |-> 0)
+  **  (CharPtrArray2.full strings_addr strings_size_pre rows )
+  **  (store_string substring_addr substring_l )
+  **  (PtrArray.seg data 0 output_size output_ptrs )
+  **  (PtrArray.undef_seg data output_size strings_size_pre )
+|--
+  “ ((i + 1 ) <= INT_MAX) ” 
+  &&  “ ((INT_MIN) <= (i + 1 )) ”
+.
+
+Definition filter_by_substring_safety_wit_10 := 
+forall (strings_size_pre: Z) (substring_addr: Z) (strings_addr: Z) (substring_l: (@list Z)) (rows: (@list (@list Z))) (output_rows: (@list (@list Z))) (output_ptrs: (@list Z)) (i: Z) (output_size: Z) (out: Z) (data: Z) (cur: Z) (hit: Z) (PreH1 : (0 <= i)) (PreH2 : (i < strings_size_pre)) (PreH3 : (0 <= output_size)) (PreH4 : (output_size <= (i + 1 ))) (PreH5 : (output_size = (Zlength (output_rows)))) (PreH6 : (output_size = (Zlength (output_ptrs)))) (PreH7 : (out <> 0)) (PreH8 : (data <> 0)) (PreH9 : (rows_well_formed_7 rows strings_size_pre )) (PreH10 : (problem_7_pre_z rows )) (PreH11 : (valid_string substring_l )) (PreH12 : ((string_length (substring_l)) < INT_MAX)) (PreH13 : (filter_substring_state_7 rows substring_l (i + 1 ) output_rows )) ,
+  ((( &( "i" ) )) # Int  |-> i)
+  **  ((( &( "output_size" ) )) # Int  |-> output_size)
+  **  ((( &( "strings" ) )) # Ptr  |-> strings_addr)
+  **  ((( &( "substring" ) )) # Ptr  |-> substring_addr)
+  **  ((( &( "strings_size" ) )) # Int  |-> strings_size_pre)
+  **  ((( &( "out" ) )) # Ptr  |-> out)
+  **  ((( &( "data" ) )) # Ptr  |-> data)
+  **  ((( &( "cur" ) )) # Ptr  |-> cur)
+  **  ((( &( "hit" ) )) # Ptr  |-> hit)
+  **  ((&((out)  # "<anonymous struct>" ->ₛ "data")) # Ptr  |-> data)
+  **  ((&((out)  # "<anonymous struct>" ->ₛ "size")) # Int  |-> 0)
+  **  (CharPtrArray2.full strings_addr strings_size_pre rows )
+  **  (store_string substring_addr substring_l )
+  **  (PtrArray.seg data 0 output_size output_ptrs )
+  **  (PtrArray.undef_seg data output_size strings_size_pre )
+|--
+  “ ((i + 1 ) <= INT_MAX) ” 
+  &&  “ ((INT_MIN) <= (i + 1 )) ”
+.
+
+Definition filter_by_substring_entail_wit_1 := 
+(
+forall (substring_pre: Z) (strings_size_pre: Z) (strings_pre: Z) (substring_addr: Z) (strings_addr: Z) (substring_l: (@list Z)) (rows: (@list (@list Z))) (retval: Z) (retval_2: Z) (PreH1 : (retval_2 <> 0)) (PreH2 : (retval <> 0)) (PreH3 : (0 <= ((string_length (substring_l)) + 1 ))) (PreH4 : (strings_pre = strings_addr)) (PreH5 : (substring_pre = substring_addr)) (PreH6 : (0 <= strings_size_pre)) (PreH7 : (strings_size_pre <= 100)) (PreH8 : (rows_well_formed_7 rows strings_size_pre )) (PreH9 : (problem_7_pre_z rows )) (PreH10 : (valid_string substring_l )) (PreH11 : ((string_length (substring_l)) < INT_MAX)) ,
+  (PtrArray.undef_seg retval_2 0 strings_size_pre )
+  **  ((&((retval)  # "<anonymous struct>" ->ₛ "data")) # Ptr  |-> retval_2)
+  **  ((&((retval)  # "<anonymous struct>" ->ₛ "size")) # Int  |-> 0)
+  **  (CharArray.full substring_pre ((string_length (substring_l)) + 1 ) (c_string (substring_l)) )
+  **  ((( &( "substring" ) )) # Ptr  |-> substring_pre)
+  **  ((( &( "strings" ) )) # Ptr  |-> strings_pre)
+  **  (CharPtrArray2.full strings_pre strings_size_pre rows )
+|--
+  EX (output_ptrs: (@list Z))  (output_rows: (@list (@list Z))) ,
+  “ (0 <= 0) ” 
+  &&  “ (0 <= strings_size_pre) ” 
+  &&  “ (0 <= 0) ” 
+  &&  “ (0 <= 0) ” 
+  &&  “ (0 = (Zlength (output_rows))) ” 
+  &&  “ (0 = (Zlength (output_ptrs))) ” 
+  &&  “ (retval <> 0) ” 
+  &&  “ (retval_2 <> 0) ” 
+  &&  “ (rows_well_formed_7 rows strings_size_pre ) ” 
+  &&  “ (problem_7_pre_z rows ) ” 
+  &&  “ (valid_string substring_l ) ” 
+  &&  “ ((string_length (substring_l)) < INT_MAX) ” 
+  &&  “ (filter_substring_state_7 rows substring_l 0 output_rows ) ”
+  &&  ((( &( "strings" ) )) # Ptr  |-> strings_addr)
+  **  ((( &( "substring" ) )) # Ptr  |-> substring_addr)
+  **  ((&((retval)  # "<anonymous struct>" ->ₛ "data")) # Ptr  |-> retval_2)
+  **  ((&((retval)  # "<anonymous struct>" ->ₛ "size")) # Int  |-> 0)
+  **  (CharPtrArray2.full strings_addr strings_size_pre rows )
+  **  (store_string substring_addr substring_l )
+  **  (PtrArray.seg retval_2 0 0 output_ptrs )
+  **  (PtrArray.undef_seg retval_2 0 strings_size_pre )
+) \/
+(
+forall (substring_pre: Z) (strings_size_pre: Z) (strings_pre: Z) (substring_addr: Z) (strings_addr: Z) (substring_l: (@list Z)) (rows: (@list (@list Z))) (retval: Z) (retval_2: Z) (PreH1 : (retval_2 <> 0)) (PreH2 : (retval <> 0)) (PreH3 : (0 <= ((string_length (substring_l)) + 1 ))) (PreH4 : (strings_pre = strings_addr)) (PreH5 : (substring_pre = substring_addr)) (PreH6 : (0 <= strings_size_pre)) (PreH7 : (strings_size_pre <= 100)) (PreH8 : (rows_well_formed_7 rows strings_size_pre )) (PreH9 : (problem_7_pre_z rows )) (PreH10 : (valid_string substring_l )) (PreH11 : ((string_length (substring_l)) < INT_MAX)) ,
+  (CharArray.full substring_pre ((string_length (substring_l)) + 1 ) (c_string (substring_l)) )
+  **  (CharPtrArray2.full strings_pre strings_size_pre rows )
+|--
+  EX (output_rows: (@list (@list Z))) ,
+  “ (strings_pre = strings_addr) ” 
+  &&  “ (substring_pre = substring_addr) ” 
+  &&  “ (0 <= 0) ” 
+  &&  “ (0 <= strings_size_pre) ” 
+  &&  “ (0 <= 0) ” 
+  &&  “ (0 <= 0) ” 
+  &&  “ (0 = (Zlength (output_rows))) ” 
+  &&  “ (0 = (Zlength ((@nil Z)))) ” 
+  &&  “ (retval <> 0) ” 
+  &&  “ (retval_2 <> 0) ” 
+  &&  “ (rows_well_formed_7 rows strings_size_pre ) ” 
+  &&  “ (problem_7_pre_z rows ) ” 
+  &&  “ (valid_string substring_l ) ” 
+  &&  “ ((string_length (substring_l)) < INT_MAX) ” 
+  &&  “ (filter_substring_state_7 rows substring_l 0 output_rows ) ”
+  &&  (CharArray.full substring_addr ((string_length (substring_l)) + 1 ) (c_string (substring_l)) )
+  **  (CharPtrArray2.full strings_addr strings_size_pre rows )
+).
+
+Definition filter_by_substring_entail_wit_2 := 
+(
+forall (strings_size_pre: Z) (substring_addr: Z) (strings_addr: Z) (substring_l: (@list Z)) (rows: (@list (@list Z))) (data: Z) (out: Z) (output_ptrs_2: (@list Z)) (output_rows_2: (@list (@list Z))) (output_size: Z) (i: Z) (PreH1 : (i < strings_size_pre)) (PreH2 : (0 <= i)) (PreH3 : (i <= strings_size_pre)) (PreH4 : (0 <= output_size)) (PreH5 : (output_size <= i)) (PreH6 : (output_size = (Zlength (output_rows_2)))) (PreH7 : (output_size = (Zlength (output_ptrs_2)))) (PreH8 : (out <> 0)) (PreH9 : (data <> 0)) (PreH10 : (rows_well_formed_7 rows strings_size_pre )) (PreH11 : (problem_7_pre_z rows )) (PreH12 : (valid_string substring_l )) (PreH13 : ((string_length (substring_l)) < INT_MAX)) (PreH14 : (filter_substring_state_7 rows substring_l i output_rows_2 )) ,
+  ((&((out)  # "<anonymous struct>" ->ₛ "data")) # Ptr  |-> data)
+  **  ((&((out)  # "<anonymous struct>" ->ₛ "size")) # Int  |-> 0)
+  **  (CharPtrArray2.full strings_addr strings_size_pre rows )
+  **  (store_string substring_addr substring_l )
+  **  (PtrArray.seg data 0 output_size output_ptrs_2 )
+  **  (PtrArray.undef_seg data output_size strings_size_pre )
+|--
+  EX (row_ptr: Z)  (output_ptrs: (@list Z))  (output_rows: (@list (@list Z))) ,
+  “ (0 <= i) ” 
+  &&  “ (i < strings_size_pre) ” 
+  &&  “ (0 <= output_size) ” 
+  &&  “ (output_size <= i) ” 
+  &&  “ (output_size = (Zlength (output_rows))) ” 
+  &&  “ (output_size = (Zlength (output_ptrs))) ” 
+  &&  “ (out <> 0) ” 
+  &&  “ (data <> 0) ” 
+  &&  “ (rows_well_formed_7 rows strings_size_pre ) ” 
+  &&  “ (row_well_formed_7 (Znth (i) (rows) ((@nil Z))) ) ” 
+  &&  “ (problem_7_pre_z rows ) ” 
+  &&  “ (valid_string substring_l ) ” 
+  &&  “ ((string_length (substring_l)) < INT_MAX) ” 
+  &&  “ (filter_substring_state_7 rows substring_l i output_rows ) ”
+  &&  ((&((out)  # "<anonymous struct>" ->ₛ "data")) # Ptr  |-> data)
+  **  ((&((out)  # "<anonymous struct>" ->ₛ "size")) # Int  |-> 0)
+  **  (CharPtrArray2.missing_i strings_addr strings_size_pre i row_ptr rows )
+  **  (((strings_addr + (i * sizeof(PTR) ) )) # Ptr  |-> row_ptr)
+  **  (store_string row_ptr (row_payload_z_7 ((Znth (i) (rows) ((@nil Z))))) )
+  **  (store_string substring_addr substring_l )
+  **  (PtrArray.seg data 0 output_size output_ptrs )
+  **  (PtrArray.undef_seg data output_size strings_size_pre )
+) \/
+(
+forall (strings_size_pre: Z) (substring_l: (@list Z)) (rows: (@list (@list Z))) (data: Z) (out: Z) (output_ptrs_2: (@list Z)) (output_rows_2: (@list (@list Z))) (output_size: Z) (i: Z) (row_ptr_2: Z)  __default__List_Z (PreH1 : (0 <= ((string_length (substring_l)) + 1 ))) (PreH2 : (0 <= (Zlength ((Znth i rows __default__List_Z))))) (PreH3 : (i < strings_size_pre)) (PreH4 : (0 <= i)) (PreH5 : (i <= strings_size_pre)) (PreH6 : (0 <= output_size)) (PreH7 : (output_size <= i)) (PreH8 : (output_size = (Zlength (output_rows_2)))) (PreH9 : (output_size = (Zlength (output_ptrs_2)))) (PreH10 : (out <> 0)) (PreH11 : (data <> 0)) (PreH12 : (rows_well_formed_7 rows strings_size_pre )) (PreH13 : (problem_7_pre_z rows )) (PreH14 : (valid_string substring_l )) (PreH15 : ((string_length (substring_l)) < INT_MAX)) (PreH16 : (filter_substring_state_7 rows substring_l i output_rows_2 )) ,
+  (CharArray.full row_ptr_2 (Zlength ((Znth i rows __default__List_Z))) (Znth i rows __default__List_Z) )
+|--
+  EX (output_rows: (@list (@list Z))) ,
+  “ (0 <= i) ” 
+  &&  “ (i < strings_size_pre) ” 
+  &&  “ (0 <= output_size) ” 
+  &&  “ (output_size <= i) ” 
+  &&  “ (output_size = (Zlength (output_rows))) ” 
+  &&  “ (output_size = (Zlength (output_ptrs_2))) ” 
+  &&  “ (out <> 0) ” 
+  &&  “ (data <> 0) ” 
+  &&  “ (rows_well_formed_7 rows strings_size_pre ) ” 
+  &&  “ (row_well_formed_7 (Znth (i) (rows) ((@nil Z))) ) ” 
+  &&  “ (problem_7_pre_z rows ) ” 
+  &&  “ (valid_string substring_l ) ” 
+  &&  “ ((string_length (substring_l)) < INT_MAX) ” 
+  &&  “ (filter_substring_state_7 rows substring_l i output_rows ) ”
+  &&  (CharArray.full row_ptr_2 ((string_length ((row_payload_z_7 ((Znth (i) (rows) ((@nil Z))))))) + 1 ) (c_string ((row_payload_z_7 ((Znth (i) (rows) ((@nil Z))))))) )
+).
+
+Definition filter_by_substring_entail_wit_3 := 
+(
+forall (strings_size_pre: Z) (substring_addr: Z) (strings_addr: Z) (substring_l: (@list Z)) (rows: (@list (@list Z))) (row_ptr: Z) (output_rows_2: (@list (@list Z))) (output_ptrs_2: (@list Z)) (i: Z) (output_size: Z) (out: Z) (data: Z) (retval: Z) (PreH1 : (retval <> 0)) (PreH2 : (strstr_result (row_payload_z_7 ((Znth (i) (rows) ((@nil Z))))) substring_l retval row_ptr )) (PreH3 : (0 <= ((string_length (substring_l)) + 1 ))) (PreH4 : (0 <= ((string_length ((row_payload_z_7 ((Znth (i) (rows) ((@nil Z))))))) + 1 ))) (PreH5 : (0 <= i)) (PreH6 : (i < strings_size_pre)) (PreH7 : (0 <= output_size)) (PreH8 : (output_size <= i)) (PreH9 : (output_size = (Zlength (output_rows_2)))) (PreH10 : (output_size = (Zlength (output_ptrs_2)))) (PreH11 : (out <> 0)) (PreH12 : (data <> 0)) (PreH13 : (rows_well_formed_7 rows strings_size_pre )) (PreH14 : (row_well_formed_7 (Znth (i) (rows) ((@nil Z))) )) (PreH15 : (problem_7_pre_z rows )) (PreH16 : (valid_string substring_l )) (PreH17 : ((string_length (substring_l)) < INT_MAX)) (PreH18 : (filter_substring_state_7 rows substring_l i output_rows_2 )) ,
+  (store_string row_ptr (row_payload_z_7 ((Znth (i) (rows) ((@nil Z))))) )
+  **  (store_string substring_addr substring_l )
+  **  ((&((out)  # "<anonymous struct>" ->ₛ "data")) # Ptr  |-> data)
+  **  ((&((out)  # "<anonymous struct>" ->ₛ "size")) # Int  |-> 0)
+  **  (CharPtrArray2.missing_i strings_addr strings_size_pre i row_ptr rows )
+  **  (((strings_addr + (i * sizeof(PTR) ) )) # Ptr  |-> row_ptr)
+  **  (PtrArray.seg data 0 output_size output_ptrs_2 )
+  **  (PtrArray.undef_seg data output_size strings_size_pre )
+|--
+  EX (output_ptrs: (@list Z))  (output_rows: (@list (@list Z))) ,
+  “ (0 <= i) ” 
+  &&  “ (i < strings_size_pre) ” 
+  &&  “ (0 <= output_size) ” 
+  &&  “ (output_size <= i) ” 
+  &&  “ (output_size = (Zlength (output_rows))) ” 
+  &&  “ (output_size = (Zlength (output_ptrs))) ” 
+  &&  “ (retval <> 0) ” 
+  &&  “ (out <> 0) ” 
+  &&  “ (data <> 0) ” 
+  &&  “ (rows_well_formed_7 rows strings_size_pre ) ” 
+  &&  “ (problem_7_pre_z rows ) ” 
+  &&  “ (valid_string substring_l ) ” 
+  &&  “ ((string_length (substring_l)) < INT_MAX) ” 
+  &&  “ (filter_substring_state_7 rows substring_l i output_rows ) ” 
+  &&  “ (substring_hit_z_7 (row_payload_z_7 ((Znth (i) (rows) ((@nil Z))))) substring_l ) ”
+  &&  ((&((out)  # "<anonymous struct>" ->ₛ "data")) # Ptr  |-> data)
+  **  ((&((out)  # "<anonymous struct>" ->ₛ "size")) # Int  |-> 0)
+  **  (CharPtrArray2.missing_i strings_addr strings_size_pre i row_ptr rows )
+  **  (((strings_addr + (i * sizeof(PTR) ) )) # Ptr  |-> row_ptr)
+  **  (store_string row_ptr (row_payload_z_7 ((Znth (i) (rows) ((@nil Z))))) )
+  **  (store_string substring_addr substring_l )
+  **  (PtrArray.seg data 0 output_size output_ptrs )
+  **  (PtrArray.undef_seg data output_size strings_size_pre )
+) \/
+(
+forall (strings_size_pre: Z) (substring_l: (@list Z)) (rows: (@list (@list Z))) (row_ptr: Z) (output_rows_2: (@list (@list Z))) (output_ptrs_2: (@list Z)) (i: Z) (output_size: Z) (out: Z) (data: Z) (retval: Z) (PreH1 : (retval <> 0)) (PreH2 : (strstr_result (row_payload_z_7 ((Znth (i) (rows) ((@nil Z))))) substring_l retval row_ptr )) (PreH3 : (0 <= ((string_length (substring_l)) + 1 ))) (PreH4 : (0 <= ((string_length ((row_payload_z_7 ((Znth (i) (rows) ((@nil Z))))))) + 1 ))) (PreH5 : (0 <= i)) (PreH6 : (i < strings_size_pre)) (PreH7 : (0 <= output_size)) (PreH8 : (output_size <= i)) (PreH9 : (output_size = (Zlength (output_rows_2)))) (PreH10 : (output_size = (Zlength (output_ptrs_2)))) (PreH11 : (out <> 0)) (PreH12 : (data <> 0)) (PreH13 : (rows_well_formed_7 rows strings_size_pre )) (PreH14 : (row_well_formed_7 (Znth (i) (rows) ((@nil Z))) )) (PreH15 : (problem_7_pre_z rows )) (PreH16 : (valid_string substring_l )) (PreH17 : ((string_length (substring_l)) < INT_MAX)) (PreH18 : (filter_substring_state_7 rows substring_l i output_rows_2 )) ,
+  TT && emp 
+|--
+  EX (output_rows: (@list (@list Z))) ,
+  “ (0 <= i) ” 
+  &&  “ (i < strings_size_pre) ” 
+  &&  “ (0 <= output_size) ” 
+  &&  “ (output_size <= i) ” 
+  &&  “ (output_size = (Zlength (output_rows))) ” 
+  &&  “ (output_size = (Zlength (output_ptrs_2))) ” 
+  &&  “ (retval <> 0) ” 
+  &&  “ (out <> 0) ” 
+  &&  “ (data <> 0) ” 
+  &&  “ (rows_well_formed_7 rows strings_size_pre ) ” 
+  &&  “ (problem_7_pre_z rows ) ” 
+  &&  “ (valid_string substring_l ) ” 
+  &&  “ ((string_length (substring_l)) < INT_MAX) ” 
+  &&  “ (filter_substring_state_7 rows substring_l i output_rows ) ” 
+  &&  “ (substring_hit_z_7 (row_payload_z_7 ((Znth (i) (rows) ((@nil Z))))) substring_l ) ”
+  &&  emp
+).
+
+Definition filter_by_substring_entail_wit_4 := 
+(
+forall (strings_size_pre: Z) (substring_addr: Z) (strings_addr: Z) (substring_l: (@list Z)) (rows: (@list (@list Z))) (row_ptr: Z) (output_rows_2: (@list (@list Z))) (output_ptrs_2: (@list Z)) (i: Z) (output_size: Z) (hit: Z) (out: Z) (data: Z) (PreH1 : (0 <= ((string_length (substring_l)) + 1 ))) (PreH2 : (0 <= ((string_length ((row_payload_z_7 ((Znth (i) (rows) ((@nil Z))))))) + 1 ))) (PreH3 : (0 <= i)) (PreH4 : (i < strings_size_pre)) (PreH5 : (0 <= output_size)) (PreH6 : (output_size <= i)) (PreH7 : (output_size = (Zlength (output_rows_2)))) (PreH8 : (output_size = (Zlength (output_ptrs_2)))) (PreH9 : (hit <> 0)) (PreH10 : (out <> 0)) (PreH11 : (data <> 0)) (PreH12 : (rows_well_formed_7 rows strings_size_pre )) (PreH13 : (problem_7_pre_z rows )) (PreH14 : (valid_string substring_l )) (PreH15 : ((string_length (substring_l)) < INT_MAX)) (PreH16 : (filter_substring_state_7 rows substring_l i output_rows_2 )) (PreH17 : (substring_hit_z_7 (row_payload_z_7 ((Znth (i) (rows) ((@nil Z))))) substring_l )) ,
+  (PtrArray.seg data 0 (output_size + 1 ) (app (output_ptrs_2) ((cons (row_ptr) ((@nil Z))))) )
+  **  (PtrArray.undef_seg data (output_size + 1 ) strings_size_pre )
+  **  (CharArray.full substring_addr ((string_length (substring_l)) + 1 ) (c_string (substring_l)) )
+  **  (CharArray.full row_ptr ((string_length ((row_payload_z_7 ((Znth (i) (rows) ((@nil Z))))))) + 1 ) (c_string ((row_payload_z_7 ((Znth (i) (rows) ((@nil Z))))))) )
+  **  ((&((out)  # "<anonymous struct>" ->ₛ "data")) # Ptr  |-> data)
+  **  ((&((out)  # "<anonymous struct>" ->ₛ "size")) # Int  |-> 0)
+  **  (CharPtrArray2.missing_i strings_addr strings_size_pre i row_ptr rows )
+  **  (((strings_addr + (i * sizeof(PTR) ) )) # Ptr  |-> row_ptr)
+|--
+  EX (output_ptrs: (@list Z))  (output_rows: (@list (@list Z))) ,
+  “ (0 <= i) ” 
+  &&  “ (i < strings_size_pre) ” 
+  &&  “ (0 <= (output_size + 1 )) ” 
+  &&  “ ((output_size + 1 ) <= (i + 1 )) ” 
+  &&  “ ((output_size + 1 ) = (Zlength (output_rows))) ” 
+  &&  “ ((output_size + 1 ) = (Zlength (output_ptrs))) ” 
+  &&  “ (out <> 0) ” 
+  &&  “ (data <> 0) ” 
+  &&  “ (rows_well_formed_7 rows strings_size_pre ) ” 
+  &&  “ (problem_7_pre_z rows ) ” 
+  &&  “ (valid_string substring_l ) ” 
+  &&  “ ((string_length (substring_l)) < INT_MAX) ” 
+  &&  “ (filter_substring_state_7 rows substring_l (i + 1 ) output_rows ) ”
+  &&  ((&((out)  # "<anonymous struct>" ->ₛ "data")) # Ptr  |-> data)
+  **  ((&((out)  # "<anonymous struct>" ->ₛ "size")) # Int  |-> 0)
+  **  (CharPtrArray2.full strings_addr strings_size_pre rows )
+  **  (store_string substring_addr substring_l )
+  **  (PtrArray.seg data 0 (output_size + 1 ) output_ptrs )
+  **  (PtrArray.undef_seg data (output_size + 1 ) strings_size_pre )
+) \/
+(
+forall (strings_size_pre: Z) (strings_addr: Z) (substring_l: (@list Z)) (rows: (@list (@list Z))) (row_ptr: Z) (output_rows_2: (@list (@list Z))) (output_ptrs_2: (@list Z)) (i: Z) (output_size: Z) (hit: Z) (out: Z) (data: Z) (PreH1 : (0 <= ((string_length (substring_l)) + 1 ))) (PreH2 : (0 <= ((string_length ((row_payload_z_7 ((Znth (i) (rows) ((@nil Z))))))) + 1 ))) (PreH3 : (0 <= i)) (PreH4 : (i < strings_size_pre)) (PreH5 : (0 <= output_size)) (PreH6 : (output_size <= i)) (PreH7 : (output_size = (Zlength (output_rows_2)))) (PreH8 : (output_size = (Zlength (output_ptrs_2)))) (PreH9 : (hit <> 0)) (PreH10 : (out <> 0)) (PreH11 : (data <> 0)) (PreH12 : (rows_well_formed_7 rows strings_size_pre )) (PreH13 : (problem_7_pre_z rows )) (PreH14 : (valid_string substring_l )) (PreH15 : ((string_length (substring_l)) < INT_MAX)) (PreH16 : (filter_substring_state_7 rows substring_l i output_rows_2 )) (PreH17 : (substring_hit_z_7 (row_payload_z_7 ((Znth (i) (rows) ((@nil Z))))) substring_l )) ,
+  (CharArray.full row_ptr ((string_length ((row_payload_z_7 ((Znth (i) (rows) ((@nil Z))))))) + 1 ) (c_string ((row_payload_z_7 ((Znth (i) (rows) ((@nil Z))))))) )
+  **  (CharPtrArray2.missing_i strings_addr strings_size_pre i row_ptr rows )
+  **  (((strings_addr + (i * sizeof(PTR) ) )) # Ptr  |-> row_ptr)
+|--
+  EX (output_rows: (@list (@list Z))) ,
+  “ (0 <= i) ” 
+  &&  “ (i < strings_size_pre) ” 
+  &&  “ (0 <= (output_size + 1 )) ” 
+  &&  “ ((output_size + 1 ) <= (i + 1 )) ” 
+  &&  “ ((output_size + 1 ) = (Zlength (output_rows))) ” 
+  &&  “ ((output_size + 1 ) = (Zlength ((app (output_ptrs_2) ((cons (row_ptr) ((@nil Z)))))))) ” 
+  &&  “ (out <> 0) ” 
+  &&  “ (data <> 0) ” 
+  &&  “ (rows_well_formed_7 rows strings_size_pre ) ” 
+  &&  “ (problem_7_pre_z rows ) ” 
+  &&  “ (valid_string substring_l ) ” 
+  &&  “ ((string_length (substring_l)) < INT_MAX) ” 
+  &&  “ (filter_substring_state_7 rows substring_l (i + 1 ) output_rows ) ”
+  &&  (CharPtrArray2.full strings_addr strings_size_pre rows )
+).
+
+Definition filter_by_substring_entail_wit_5 := 
+(
+forall (strings_size_pre: Z) (substring_addr: Z) (strings_addr: Z) (substring_l: (@list Z)) (rows: (@list (@list Z))) (row_ptr: Z) (output_rows_2: (@list (@list Z))) (output_ptrs_2: (@list Z)) (i: Z) (output_size: Z) (out: Z) (data: Z) (retval: Z) (PreH1 : (retval = 0)) (PreH2 : (strstr_result (row_payload_z_7 ((Znth (i) (rows) ((@nil Z))))) substring_l retval row_ptr )) (PreH3 : (0 <= ((string_length (substring_l)) + 1 ))) (PreH4 : (0 <= ((string_length ((row_payload_z_7 ((Znth (i) (rows) ((@nil Z))))))) + 1 ))) (PreH5 : (0 <= i)) (PreH6 : (i < strings_size_pre)) (PreH7 : (0 <= output_size)) (PreH8 : (output_size <= i)) (PreH9 : (output_size = (Zlength (output_rows_2)))) (PreH10 : (output_size = (Zlength (output_ptrs_2)))) (PreH11 : (out <> 0)) (PreH12 : (data <> 0)) (PreH13 : (rows_well_formed_7 rows strings_size_pre )) (PreH14 : (row_well_formed_7 (Znth (i) (rows) ((@nil Z))) )) (PreH15 : (problem_7_pre_z rows )) (PreH16 : (valid_string substring_l )) (PreH17 : ((string_length (substring_l)) < INT_MAX)) (PreH18 : (filter_substring_state_7 rows substring_l i output_rows_2 )) ,
+  (store_string row_ptr (row_payload_z_7 ((Znth (i) (rows) ((@nil Z))))) )
+  **  (store_string substring_addr substring_l )
+  **  ((&((out)  # "<anonymous struct>" ->ₛ "data")) # Ptr  |-> data)
+  **  ((&((out)  # "<anonymous struct>" ->ₛ "size")) # Int  |-> 0)
+  **  (CharPtrArray2.missing_i strings_addr strings_size_pre i row_ptr rows )
+  **  (((strings_addr + (i * sizeof(PTR) ) )) # Ptr  |-> row_ptr)
+  **  (PtrArray.seg data 0 output_size output_ptrs_2 )
+  **  (PtrArray.undef_seg data output_size strings_size_pre )
+|--
+  EX (output_ptrs: (@list Z))  (output_rows: (@list (@list Z))) ,
+  “ (0 <= i) ” 
+  &&  “ (i < strings_size_pre) ” 
+  &&  “ (0 <= output_size) ” 
+  &&  “ (output_size <= i) ” 
+  &&  “ (output_size = (Zlength (output_rows))) ” 
+  &&  “ (output_size = (Zlength (output_ptrs))) ” 
+  &&  “ (retval = 0) ” 
+  &&  “ (out <> 0) ” 
+  &&  “ (data <> 0) ” 
+  &&  “ (rows_well_formed_7 rows strings_size_pre ) ” 
+  &&  “ (problem_7_pre_z rows ) ” 
+  &&  “ (valid_string substring_l ) ” 
+  &&  “ ((string_length (substring_l)) < INT_MAX) ” 
+  &&  “ (filter_substring_state_7 rows substring_l i output_rows ) ” 
+  &&  “ (substring_miss_z_7 (row_payload_z_7 ((Znth (i) (rows) ((@nil Z))))) substring_l ) ”
+  &&  ((&((out)  # "<anonymous struct>" ->ₛ "data")) # Ptr  |-> data)
+  **  ((&((out)  # "<anonymous struct>" ->ₛ "size")) # Int  |-> 0)
+  **  (CharPtrArray2.missing_i strings_addr strings_size_pre i row_ptr rows )
+  **  (((strings_addr + (i * sizeof(PTR) ) )) # Ptr  |-> row_ptr)
+  **  (store_string row_ptr (row_payload_z_7 ((Znth (i) (rows) ((@nil Z))))) )
+  **  (store_string substring_addr substring_l )
+  **  (PtrArray.seg data 0 output_size output_ptrs )
+  **  (PtrArray.undef_seg data output_size strings_size_pre )
+) \/
+(
+forall (strings_size_pre: Z) (substring_l: (@list Z)) (rows: (@list (@list Z))) (row_ptr: Z) (output_rows_2: (@list (@list Z))) (output_ptrs_2: (@list Z)) (i: Z) (output_size: Z) (out: Z) (data: Z) (retval: Z) (PreH1 : (retval = 0)) (PreH2 : (strstr_result (row_payload_z_7 ((Znth (i) (rows) ((@nil Z))))) substring_l retval row_ptr )) (PreH3 : (0 <= ((string_length (substring_l)) + 1 ))) (PreH4 : (0 <= ((string_length ((row_payload_z_7 ((Znth (i) (rows) ((@nil Z))))))) + 1 ))) (PreH5 : (0 <= i)) (PreH6 : (i < strings_size_pre)) (PreH7 : (0 <= output_size)) (PreH8 : (output_size <= i)) (PreH9 : (output_size = (Zlength (output_rows_2)))) (PreH10 : (output_size = (Zlength (output_ptrs_2)))) (PreH11 : (out <> 0)) (PreH12 : (data <> 0)) (PreH13 : (rows_well_formed_7 rows strings_size_pre )) (PreH14 : (row_well_formed_7 (Znth (i) (rows) ((@nil Z))) )) (PreH15 : (problem_7_pre_z rows )) (PreH16 : (valid_string substring_l )) (PreH17 : ((string_length (substring_l)) < INT_MAX)) (PreH18 : (filter_substring_state_7 rows substring_l i output_rows_2 )) ,
+  TT && emp 
+|--
+  EX (output_rows: (@list (@list Z))) ,
+  “ (0 <= i) ” 
+  &&  “ (i < strings_size_pre) ” 
+  &&  “ (0 <= output_size) ” 
+  &&  “ (output_size <= i) ” 
+  &&  “ (output_size = (Zlength (output_rows))) ” 
+  &&  “ (output_size = (Zlength (output_ptrs_2))) ” 
+  &&  “ (retval = 0) ” 
+  &&  “ (out <> 0) ” 
+  &&  “ (data <> 0) ” 
+  &&  “ (rows_well_formed_7 rows strings_size_pre ) ” 
+  &&  “ (problem_7_pre_z rows ) ” 
+  &&  “ (valid_string substring_l ) ” 
+  &&  “ ((string_length (substring_l)) < INT_MAX) ” 
+  &&  “ (filter_substring_state_7 rows substring_l i output_rows ) ” 
+  &&  “ (substring_miss_z_7 (row_payload_z_7 ((Znth (i) (rows) ((@nil Z))))) substring_l ) ”
+  &&  emp
+).
+
+Definition filter_by_substring_entail_wit_6 := 
+(
+forall (strings_size_pre: Z) (substring_addr: Z) (strings_addr: Z) (substring_l: (@list Z)) (rows: (@list (@list Z))) (row_ptr: Z) (output_rows_2: (@list (@list Z))) (output_ptrs_2: (@list Z)) (i: Z) (output_size: Z) (hit: Z) (out: Z) (data: Z) (PreH1 : (0 <= i)) (PreH2 : (i < strings_size_pre)) (PreH3 : (0 <= output_size)) (PreH4 : (output_size <= i)) (PreH5 : (output_size = (Zlength (output_rows_2)))) (PreH6 : (output_size = (Zlength (output_ptrs_2)))) (PreH7 : (hit = 0)) (PreH8 : (out <> 0)) (PreH9 : (data <> 0)) (PreH10 : (rows_well_formed_7 rows strings_size_pre )) (PreH11 : (problem_7_pre_z rows )) (PreH12 : (valid_string substring_l )) (PreH13 : ((string_length (substring_l)) < INT_MAX)) (PreH14 : (filter_substring_state_7 rows substring_l i output_rows_2 )) (PreH15 : (substring_miss_z_7 (row_payload_z_7 ((Znth (i) (rows) ((@nil Z))))) substring_l )) ,
+  ((&((out)  # "<anonymous struct>" ->ₛ "data")) # Ptr  |-> data)
+  **  ((&((out)  # "<anonymous struct>" ->ₛ "size")) # Int  |-> 0)
+  **  (CharPtrArray2.missing_i strings_addr strings_size_pre i row_ptr rows )
+  **  (((strings_addr + (i * sizeof(PTR) ) )) # Ptr  |-> row_ptr)
+  **  (store_string row_ptr (row_payload_z_7 ((Znth (i) (rows) ((@nil Z))))) )
+  **  (store_string substring_addr substring_l )
+  **  (PtrArray.seg data 0 output_size output_ptrs_2 )
+  **  (PtrArray.undef_seg data output_size strings_size_pre )
+|--
+  EX (output_ptrs: (@list Z))  (output_rows: (@list (@list Z))) ,
+  “ (0 <= i) ” 
+  &&  “ (i < strings_size_pre) ” 
+  &&  “ (0 <= output_size) ” 
+  &&  “ (output_size <= (i + 1 )) ” 
+  &&  “ (output_size = (Zlength (output_rows))) ” 
+  &&  “ (output_size = (Zlength (output_ptrs))) ” 
+  &&  “ (out <> 0) ” 
+  &&  “ (data <> 0) ” 
+  &&  “ (rows_well_formed_7 rows strings_size_pre ) ” 
+  &&  “ (problem_7_pre_z rows ) ” 
+  &&  “ (valid_string substring_l ) ” 
+  &&  “ ((string_length (substring_l)) < INT_MAX) ” 
+  &&  “ (filter_substring_state_7 rows substring_l (i + 1 ) output_rows ) ”
+  &&  ((&((out)  # "<anonymous struct>" ->ₛ "data")) # Ptr  |-> data)
+  **  ((&((out)  # "<anonymous struct>" ->ₛ "size")) # Int  |-> 0)
+  **  (CharPtrArray2.full strings_addr strings_size_pre rows )
+  **  (store_string substring_addr substring_l )
+  **  (PtrArray.seg data 0 output_size output_ptrs )
+  **  (PtrArray.undef_seg data output_size strings_size_pre )
+) \/
+(
+forall (strings_size_pre: Z) (strings_addr: Z) (substring_l: (@list Z)) (rows: (@list (@list Z))) (row_ptr: Z) (output_rows_2: (@list (@list Z))) (output_ptrs_2: (@list Z)) (i: Z) (output_size: Z) (hit: Z) (out: Z) (data: Z) (PreH1 : (0 <= ((string_length (substring_l)) + 1 ))) (PreH2 : (0 <= ((string_length ((row_payload_z_7 ((Znth (i) (rows) ((@nil Z))))))) + 1 ))) (PreH3 : (0 <= i)) (PreH4 : (i < strings_size_pre)) (PreH5 : (0 <= output_size)) (PreH6 : (output_size <= i)) (PreH7 : (output_size = (Zlength (output_rows_2)))) (PreH8 : (output_size = (Zlength (output_ptrs_2)))) (PreH9 : (hit = 0)) (PreH10 : (out <> 0)) (PreH11 : (data <> 0)) (PreH12 : (rows_well_formed_7 rows strings_size_pre )) (PreH13 : (problem_7_pre_z rows )) (PreH14 : (valid_string substring_l )) (PreH15 : ((string_length (substring_l)) < INT_MAX)) (PreH16 : (filter_substring_state_7 rows substring_l i output_rows_2 )) (PreH17 : (substring_miss_z_7 (row_payload_z_7 ((Znth (i) (rows) ((@nil Z))))) substring_l )) ,
+  (CharArray.full row_ptr ((string_length ((row_payload_z_7 ((Znth (i) (rows) ((@nil Z))))))) + 1 ) (c_string ((row_payload_z_7 ((Znth (i) (rows) ((@nil Z))))))) )
+  **  (CharPtrArray2.missing_i strings_addr strings_size_pre i row_ptr rows )
+  **  (((strings_addr + (i * sizeof(PTR) ) )) # Ptr  |-> row_ptr)
+|--
+  EX (output_rows: (@list (@list Z))) ,
+  “ (0 <= i) ” 
+  &&  “ (i < strings_size_pre) ” 
+  &&  “ (0 <= output_size) ” 
+  &&  “ (output_size <= (i + 1 )) ” 
+  &&  “ (output_size = (Zlength (output_rows))) ” 
+  &&  “ (output_size = (Zlength (output_ptrs_2))) ” 
+  &&  “ (out <> 0) ” 
+  &&  “ (data <> 0) ” 
+  &&  “ (rows_well_formed_7 rows strings_size_pre ) ” 
+  &&  “ (problem_7_pre_z rows ) ” 
+  &&  “ (valid_string substring_l ) ” 
+  &&  “ ((string_length (substring_l)) < INT_MAX) ” 
+  &&  “ (filter_substring_state_7 rows substring_l (i + 1 ) output_rows ) ”
+  &&  (CharPtrArray2.full strings_addr strings_size_pre rows )
+).
+
+Definition filter_by_substring_entail_wit_7_1 := 
+forall (strings_size_pre: Z) (substring_addr: Z) (strings_addr: Z) (substring_l: (@list Z)) (rows: (@list (@list Z))) (output_rows_2: (@list (@list Z))) (output_ptrs_2: (@list Z)) (i: Z) (output_size: Z) (out: Z) (data: Z) (PreH1 : (0 <= i)) (PreH2 : (i < strings_size_pre)) (PreH3 : (0 <= output_size)) (PreH4 : (output_size <= (i + 1 ))) (PreH5 : (output_size = (Zlength (output_rows_2)))) (PreH6 : (output_size = (Zlength (output_ptrs_2)))) (PreH7 : (out <> 0)) (PreH8 : (data <> 0)) (PreH9 : (rows_well_formed_7 rows strings_size_pre )) (PreH10 : (problem_7_pre_z rows )) (PreH11 : (valid_string substring_l )) (PreH12 : ((string_length (substring_l)) < INT_MAX)) (PreH13 : (filter_substring_state_7 rows substring_l (i + 1 ) output_rows_2 )) ,
+  ((&((out)  # "<anonymous struct>" ->ₛ "data")) # Ptr  |-> data)
+  **  ((&((out)  # "<anonymous struct>" ->ₛ "size")) # Int  |-> 0)
+  **  (CharPtrArray2.full strings_addr strings_size_pre rows )
+  **  (store_string substring_addr substring_l )
+  **  (PtrArray.seg data 0 output_size output_ptrs_2 )
+  **  (PtrArray.undef_seg data output_size strings_size_pre )
+|--
+  EX (output_ptrs: (@list Z))  (output_rows: (@list (@list Z))) ,
+  “ (0 <= (i + 1 )) ” 
+  &&  “ ((i + 1 ) <= strings_size_pre) ” 
+  &&  “ (0 <= output_size) ” 
+  &&  “ (output_size <= (i + 1 )) ” 
+  &&  “ (output_size = (Zlength (output_rows))) ” 
+  &&  “ (output_size = (Zlength (output_ptrs))) ” 
+  &&  “ (out <> 0) ” 
+  &&  “ (data <> 0) ” 
+  &&  “ (rows_well_formed_7 rows strings_size_pre ) ” 
+  &&  “ (problem_7_pre_z rows ) ” 
+  &&  “ (valid_string substring_l ) ” 
+  &&  “ ((string_length (substring_l)) < INT_MAX) ” 
+  &&  “ (filter_substring_state_7 rows substring_l (i + 1 ) output_rows ) ”
+  &&  ((&((out)  # "<anonymous struct>" ->ₛ "data")) # Ptr  |-> data)
+  **  ((&((out)  # "<anonymous struct>" ->ₛ "size")) # Int  |-> 0)
+  **  (CharPtrArray2.full strings_addr strings_size_pre rows )
+  **  (store_string substring_addr substring_l )
+  **  (PtrArray.seg data 0 output_size output_ptrs )
+  **  (PtrArray.undef_seg data output_size strings_size_pre )
+.
+
+Definition filter_by_substring_entail_wit_7_2 := 
+forall (strings_size_pre: Z) (substring_addr: Z) (strings_addr: Z) (substring_l: (@list Z)) (rows: (@list (@list Z))) (output_rows_2: (@list (@list Z))) (output_ptrs_2: (@list Z)) (i: Z) (output_size: Z) (out: Z) (data: Z) (PreH1 : (0 <= i)) (PreH2 : (i < strings_size_pre)) (PreH3 : (0 <= output_size)) (PreH4 : (output_size <= (i + 1 ))) (PreH5 : (output_size = (Zlength (output_rows_2)))) (PreH6 : (output_size = (Zlength (output_ptrs_2)))) (PreH7 : (out <> 0)) (PreH8 : (data <> 0)) (PreH9 : (rows_well_formed_7 rows strings_size_pre )) (PreH10 : (problem_7_pre_z rows )) (PreH11 : (valid_string substring_l )) (PreH12 : ((string_length (substring_l)) < INT_MAX)) (PreH13 : (filter_substring_state_7 rows substring_l (i + 1 ) output_rows_2 )) ,
+  ((&((out)  # "<anonymous struct>" ->ₛ "data")) # Ptr  |-> data)
+  **  ((&((out)  # "<anonymous struct>" ->ₛ "size")) # Int  |-> 0)
+  **  (CharPtrArray2.full strings_addr strings_size_pre rows )
+  **  (store_string substring_addr substring_l )
+  **  (PtrArray.seg data 0 output_size output_ptrs_2 )
+  **  (PtrArray.undef_seg data output_size strings_size_pre )
+|--
+  EX (output_ptrs: (@list Z))  (output_rows: (@list (@list Z))) ,
+  “ (0 <= (i + 1 )) ” 
+  &&  “ ((i + 1 ) <= strings_size_pre) ” 
+  &&  “ (0 <= output_size) ” 
+  &&  “ (output_size <= (i + 1 )) ” 
+  &&  “ (output_size = (Zlength (output_rows))) ” 
+  &&  “ (output_size = (Zlength (output_ptrs))) ” 
+  &&  “ (out <> 0) ” 
+  &&  “ (data <> 0) ” 
+  &&  “ (rows_well_formed_7 rows strings_size_pre ) ” 
+  &&  “ (problem_7_pre_z rows ) ” 
+  &&  “ (valid_string substring_l ) ” 
+  &&  “ ((string_length (substring_l)) < INT_MAX) ” 
+  &&  “ (filter_substring_state_7 rows substring_l (i + 1 ) output_rows ) ”
+  &&  ((&((out)  # "<anonymous struct>" ->ₛ "data")) # Ptr  |-> data)
+  **  ((&((out)  # "<anonymous struct>" ->ₛ "size")) # Int  |-> 0)
+  **  (CharPtrArray2.full strings_addr strings_size_pre rows )
+  **  (store_string substring_addr substring_l )
+  **  (PtrArray.seg data 0 output_size output_ptrs )
+  **  (PtrArray.undef_seg data output_size strings_size_pre )
+.
+
+Definition filter_by_substring_entail_wit_8 := 
+(
+forall (strings_size_pre: Z) (substring_addr: Z) (strings_addr: Z) (substring_l: (@list Z)) (rows: (@list (@list Z))) (data: Z) (out: Z) (output_ptrs_2: (@list Z)) (output_rows_2: (@list (@list Z))) (output_size: Z) (i: Z) (PreH1 : (i >= strings_size_pre)) (PreH2 : (0 <= i)) (PreH3 : (i <= strings_size_pre)) (PreH4 : (0 <= output_size)) (PreH5 : (output_size <= i)) (PreH6 : (output_size = (Zlength (output_rows_2)))) (PreH7 : (output_size = (Zlength (output_ptrs_2)))) (PreH8 : (out <> 0)) (PreH9 : (data <> 0)) (PreH10 : (rows_well_formed_7 rows strings_size_pre )) (PreH11 : (problem_7_pre_z rows )) (PreH12 : (valid_string substring_l )) (PreH13 : ((string_length (substring_l)) < INT_MAX)) (PreH14 : (filter_substring_state_7 rows substring_l i output_rows_2 )) ,
+  ((&((out)  # "<anonymous struct>" ->ₛ "data")) # Ptr  |-> data)
+  **  ((&((out)  # "<anonymous struct>" ->ₛ "size")) # Int  |-> 0)
+  **  (CharPtrArray2.full strings_addr strings_size_pre rows )
+  **  (store_string substring_addr substring_l )
+  **  (PtrArray.seg data 0 output_size output_ptrs_2 )
+  **  (PtrArray.undef_seg data output_size strings_size_pre )
+|--
+  EX (output_ptrs: (@list Z))  (output_rows: (@list (@list Z))) ,
+  “ (0 <= output_size) ” 
+  &&  “ (output_size <= strings_size_pre) ” 
+  &&  “ (output_size = (Zlength (output_rows))) ” 
+  &&  “ (output_size = (Zlength (output_ptrs))) ” 
+  &&  “ (out <> 0) ” 
+  &&  “ (data <> 0) ” 
+  &&  “ (rows_well_formed_7 rows strings_size_pre ) ” 
+  &&  “ (problem_7_pre_z rows ) ” 
+  &&  “ (valid_string substring_l ) ” 
+  &&  “ (filter_substring_state_7 rows substring_l strings_size_pre output_rows ) ” 
+  &&  “ (problem_7_spec_z rows substring_l output_rows ) ”
+  &&  ((&((out)  # "<anonymous struct>" ->ₛ "data")) # Ptr  |-> data)
+  **  ((&((out)  # "<anonymous struct>" ->ₛ "size")) # Int  |-> 0)
+  **  (CharPtrArray2.full strings_addr strings_size_pre rows )
+  **  (store_string substring_addr substring_l )
+  **  (PtrArray.seg data 0 output_size output_ptrs )
+  **  (PtrArray.undef_seg data output_size strings_size_pre )
+) \/
+(
+forall (strings_size_pre: Z) (substring_l: (@list Z)) (rows: (@list (@list Z))) (data: Z) (out: Z) (output_ptrs_2: (@list Z)) (output_rows_2: (@list (@list Z))) (output_size: Z) (i: Z) (PreH1 : (0 <= ((string_length (substring_l)) + 1 ))) (PreH2 : (i >= strings_size_pre)) (PreH3 : (0 <= i)) (PreH4 : (i <= strings_size_pre)) (PreH5 : (0 <= output_size)) (PreH6 : (output_size <= i)) (PreH7 : (output_size = (Zlength (output_rows_2)))) (PreH8 : (output_size = (Zlength (output_ptrs_2)))) (PreH9 : (out <> 0)) (PreH10 : (data <> 0)) (PreH11 : (rows_well_formed_7 rows strings_size_pre )) (PreH12 : (problem_7_pre_z rows )) (PreH13 : (valid_string substring_l )) (PreH14 : ((string_length (substring_l)) < INT_MAX)) (PreH15 : (filter_substring_state_7 rows substring_l i output_rows_2 )) ,
+  TT && emp 
+|--
+  EX (output_rows: (@list (@list Z))) ,
+  “ (0 <= output_size) ” 
+  &&  “ (output_size <= strings_size_pre) ” 
+  &&  “ (output_size = (Zlength (output_rows))) ” 
+  &&  “ (output_size = (Zlength (output_ptrs_2))) ” 
+  &&  “ (out <> 0) ” 
+  &&  “ (data <> 0) ” 
+  &&  “ (rows_well_formed_7 rows strings_size_pre ) ” 
+  &&  “ (problem_7_pre_z rows ) ” 
+  &&  “ (valid_string substring_l ) ” 
+  &&  “ (filter_substring_state_7 rows substring_l strings_size_pre output_rows ) ” 
+  &&  “ (problem_7_spec_z rows substring_l output_rows ) ”
+  &&  emp
+).
+
+Definition filter_by_substring_return_wit_1 := 
+(
+forall (strings_size_pre: Z) (substring_addr: Z) (strings_addr: Z) (substring_l: (@list Z)) (rows: (@list (@list Z))) (output_rows_2: (@list (@list Z))) (output_ptrs_2: (@list Z)) (output_size_2: Z) (out: Z) (data_2: Z) (PreH1 : (0 <= output_size_2)) (PreH2 : (output_size_2 <= strings_size_pre)) (PreH3 : (output_size_2 = (Zlength (output_rows_2)))) (PreH4 : (output_size_2 = (Zlength (output_ptrs_2)))) (PreH5 : (out <> 0)) (PreH6 : (data_2 <> 0)) (PreH7 : (rows_well_formed_7 rows strings_size_pre )) (PreH8 : (problem_7_pre_z rows )) (PreH9 : (valid_string substring_l )) (PreH10 : (filter_substring_state_7 rows substring_l strings_size_pre output_rows_2 )) (PreH11 : (problem_7_spec_z rows substring_l output_rows_2 )) ,
+  ((&((out)  # "<anonymous struct>" ->ₛ "data")) # Ptr  |-> data_2)
+  **  ((&((out)  # "<anonymous struct>" ->ₛ "size")) # Int  |-> output_size_2)
+  **  (CharPtrArray2.full strings_addr strings_size_pre rows )
+  **  (store_string substring_addr substring_l )
+  **  (PtrArray.seg data_2 0 output_size_2 output_ptrs_2 )
+  **  (PtrArray.undef_seg data_2 output_size_2 strings_size_pre )
+|--
+  EX (output_ptrs: (@list Z))  (output_rows: (@list (@list Z)))  (output_size: Z)  (data: Z) ,
+  “ (out <> 0) ” 
+  &&  “ (data <> 0) ” 
+  &&  “ (0 <= output_size) ” 
+  &&  “ (output_size <= strings_size_pre) ” 
+  &&  “ (output_size = (Zlength (output_rows))) ” 
+  &&  “ (output_size = (Zlength (output_ptrs))) ” 
+  &&  “ (problem_7_spec_z rows substring_l output_rows ) ”
+  &&  ((&((out)  # "<anonymous struct>" ->ₛ "data")) # Ptr  |-> data)
+  **  ((&((out)  # "<anonymous struct>" ->ₛ "size")) # Int  |-> output_size)
+  **  (CharPtrArray2.full strings_addr strings_size_pre rows )
+  **  (store_string substring_addr substring_l )
+  **  (PtrArray.seg data 0 output_size output_ptrs )
+  **  (PtrArray.undef_seg data output_size strings_size_pre )
+) \/
+(
+forall (strings_size_pre: Z) (substring_l: (@list Z)) (rows: (@list (@list Z))) (output_rows_2: (@list (@list Z))) (output_ptrs_2: (@list Z)) (output_size_2: Z) (out: Z) (data_2: Z) (PreH1 : (0 <= ((string_length (substring_l)) + 1 ))) (PreH2 : (0 <= output_size_2)) (PreH3 : (output_size_2 <= strings_size_pre)) (PreH4 : (output_size_2 = (Zlength (output_rows_2)))) (PreH5 : (output_size_2 = (Zlength (output_ptrs_2)))) (PreH6 : (out <> 0)) (PreH7 : (data_2 <> 0)) (PreH8 : (rows_well_formed_7 rows strings_size_pre )) (PreH9 : (problem_7_pre_z rows )) (PreH10 : (valid_string substring_l )) (PreH11 : (filter_substring_state_7 rows substring_l strings_size_pre output_rows_2 )) (PreH12 : (problem_7_spec_z rows substring_l output_rows_2 )) ,
+  (PtrArray.seg data_2 0 output_size_2 output_ptrs_2 )
+  **  (PtrArray.undef_seg data_2 output_size_2 strings_size_pre )
+|--
+  EX (output_ptrs: (@list Z))  (output_rows: (@list (@list Z))) ,
+  “ (output_size_2 = (Zlength (output_rows))) ” 
+  &&  “ (output_size_2 = (Zlength (output_rows))) ” 
+  &&  “ (out <> 0) ” 
+  &&  “ (data_2 <> 0) ” 
+  &&  “ (0 <= (Zlength (output_rows))) ” 
+  &&  “ ((Zlength (output_rows)) <= strings_size_pre) ” 
+  &&  “ ((Zlength (output_rows)) = (Zlength (output_ptrs))) ” 
+  &&  “ (problem_7_spec_z rows substring_l output_rows ) ”
+  &&  (PtrArray.seg data_2 0 (Zlength (output_rows)) output_ptrs )
+  **  (PtrArray.undef_seg data_2 (Zlength (output_rows)) strings_size_pre )
+).
+
+Definition filter_by_substring_partial_solve_wit_1 := 
+forall (substring_pre: Z) (strings_size_pre: Z) (strings_pre: Z) (substring_addr: Z) (strings_addr: Z) (substring_l: (@list Z)) (rows: (@list (@list Z))) (PreH1 : (strings_pre = strings_addr)) (PreH2 : (substring_pre = substring_addr)) (PreH3 : (0 <= strings_size_pre)) (PreH4 : (strings_size_pre <= 100)) (PreH5 : (rows_well_formed_7 rows strings_size_pre )) (PreH6 : (problem_7_pre_z rows )) (PreH7 : (valid_string substring_l )) (PreH8 : ((string_length (substring_l)) < INT_MAX)) ,
+  (CharPtrArray2.full strings_pre strings_size_pre rows )
+  **  (store_string substring_pre substring_l )
+|--
+  “ (0 <= ((string_length (substring_l)) + 1 )) ” 
+  &&  “ (strings_pre = strings_addr) ” 
+  &&  “ (substring_pre = substring_addr) ” 
+  &&  “ (0 <= strings_size_pre) ” 
+  &&  “ (strings_size_pre <= 100) ” 
+  &&  “ (rows_well_formed_7 rows strings_size_pre ) ” 
+  &&  “ (problem_7_pre_z rows ) ” 
+  &&  “ (valid_string substring_l ) ” 
+  &&  “ ((string_length (substring_l)) < INT_MAX) ”
+  &&  (CharArray.full substring_pre ((string_length (substring_l)) + 1 ) (c_string (substring_l)) )
+  **  (CharPtrArray2.full strings_pre strings_size_pre rows )
+.
+
+Definition filter_by_substring_partial_solve_wit_2_pure := 
+forall (substring_pre: Z) (strings_size_pre: Z) (strings_pre: Z) (substring_addr: Z) (strings_addr: Z) (substring_l: (@list Z)) (rows: (@list (@list Z))) (retval: Z) (PreH1 : (retval <> 0)) (PreH2 : (0 <= ((string_length (substring_l)) + 1 ))) (PreH3 : (strings_pre = strings_addr)) (PreH4 : (substring_pre = substring_addr)) (PreH5 : (0 <= strings_size_pre)) (PreH6 : (strings_size_pre <= 100)) (PreH7 : (rows_well_formed_7 rows strings_size_pre )) (PreH8 : (problem_7_pre_z rows )) (PreH9 : (valid_string substring_l )) (PreH10 : ((string_length (substring_l)) < INT_MAX)) ,
+  ((&((retval)  # "<anonymous struct>" ->ₛ "data")) # Ptr  |->_)
+  **  ((&((retval)  # "<anonymous struct>" ->ₛ "size")) # Int  |-> 0)
+  **  (CharArray.full substring_pre ((string_length (substring_l)) + 1 ) (c_string (substring_l)) )
+  **  ((( &( "out" ) )) # Ptr  |-> retval)
+  **  ((( &( "substring" ) )) # Ptr  |-> substring_pre)
+  **  ((( &( "strings_size" ) )) # Int  |-> strings_size_pre)
+  **  ((( &( "strings" ) )) # Ptr  |-> strings_pre)
+  **  (CharPtrArray2.full strings_pre strings_size_pre rows )
+|--
+  “ (0 <= strings_size_pre) ” 
+  &&  “ (strings_size_pre < INT_MAX) ”
+.
+
+Definition filter_by_substring_partial_solve_wit_2_aux := 
+forall (substring_pre: Z) (strings_size_pre: Z) (strings_pre: Z) (substring_addr: Z) (strings_addr: Z) (substring_l: (@list Z)) (rows: (@list (@list Z))) (retval: Z) (PreH1 : (retval <> 0)) (PreH2 : (0 <= ((string_length (substring_l)) + 1 ))) (PreH3 : (strings_pre = strings_addr)) (PreH4 : (substring_pre = substring_addr)) (PreH5 : (0 <= strings_size_pre)) (PreH6 : (strings_size_pre <= 100)) (PreH7 : (rows_well_formed_7 rows strings_size_pre )) (PreH8 : (problem_7_pre_z rows )) (PreH9 : (valid_string substring_l )) (PreH10 : ((string_length (substring_l)) < INT_MAX)) ,
+  ((&((retval)  # "<anonymous struct>" ->ₛ "data")) # Ptr  |->_)
+  **  ((&((retval)  # "<anonymous struct>" ->ₛ "size")) # Int  |-> 0)
+  **  (CharArray.full substring_pre ((string_length (substring_l)) + 1 ) (c_string (substring_l)) )
+  **  (CharPtrArray2.full strings_pre strings_size_pre rows )
+|--
+  “ (0 <= strings_size_pre) ” 
+  &&  “ (strings_size_pre < INT_MAX) ” 
+  &&  “ (retval <> 0) ” 
+  &&  “ (0 <= ((string_length (substring_l)) + 1 )) ” 
+  &&  “ (strings_pre = strings_addr) ” 
+  &&  “ (substring_pre = substring_addr) ” 
+  &&  “ (0 <= strings_size_pre) ” 
+  &&  “ (strings_size_pre <= 100) ” 
+  &&  “ (rows_well_formed_7 rows strings_size_pre ) ” 
+  &&  “ (problem_7_pre_z rows ) ” 
+  &&  “ (valid_string substring_l ) ” 
+  &&  “ ((string_length (substring_l)) < INT_MAX) ”
+  &&  ((&((retval)  # "<anonymous struct>" ->ₛ "data")) # Ptr  |->_)
+  **  ((&((retval)  # "<anonymous struct>" ->ₛ "size")) # Int  |-> 0)
+  **  (CharArray.full substring_pre ((string_length (substring_l)) + 1 ) (c_string (substring_l)) )
+  **  (CharPtrArray2.full strings_pre strings_size_pre rows )
+.
+
+Definition filter_by_substring_partial_solve_wit_2 := filter_by_substring_partial_solve_wit_2_pure -> filter_by_substring_partial_solve_wit_2_aux.
+
+Definition filter_by_substring_partial_solve_wit_3_pure := 
+(
+forall (strings_size_pre: Z) (substring_addr: Z) (strings_addr: Z) (substring_l: (@list Z)) (rows: (@list (@list Z))) (row_ptr: Z) (output_rows: (@list (@list Z))) (output_ptrs: (@list Z)) (i: Z) (output_size: Z) (out: Z) (data: Z) (hit: Z) (PreH1 : (0 <= i)) (PreH2 : (i < strings_size_pre)) (PreH3 : (0 <= output_size)) (PreH4 : (output_size <= i)) (PreH5 : (output_size = (Zlength (output_rows)))) (PreH6 : (output_size = (Zlength (output_ptrs)))) (PreH7 : (out <> 0)) (PreH8 : (data <> 0)) (PreH9 : (rows_well_formed_7 rows strings_size_pre )) (PreH10 : (row_well_formed_7 (Znth (i) (rows) ((@nil Z))) )) (PreH11 : (problem_7_pre_z rows )) (PreH12 : (valid_string substring_l )) (PreH13 : ((string_length (substring_l)) < INT_MAX)) (PreH14 : (filter_substring_state_7 rows substring_l i output_rows )) ,
+  ((( &( "i" ) )) # Int  |-> i)
+  **  ((( &( "output_size" ) )) # Int  |-> output_size)
+  **  ((( &( "strings" ) )) # Ptr  |-> strings_addr)
+  **  ((( &( "substring" ) )) # Ptr  |-> substring_addr)
+  **  ((( &( "strings_size" ) )) # Int  |-> strings_size_pre)
+  **  ((( &( "out" ) )) # Ptr  |-> out)
+  **  ((( &( "data" ) )) # Ptr  |-> data)
+  **  ((( &( "cur" ) )) # Ptr  |-> row_ptr)
+  **  ((( &( "hit" ) )) # Ptr  |-> hit)
+  **  ((&((out)  # "<anonymous struct>" ->ₛ "data")) # Ptr  |-> data)
+  **  ((&((out)  # "<anonymous struct>" ->ₛ "size")) # Int  |-> 0)
+  **  (CharPtrArray2.missing_i strings_addr strings_size_pre i row_ptr rows )
+  **  (((strings_addr + (i * sizeof(PTR) ) )) # Ptr  |-> row_ptr)
+  **  (store_string row_ptr (row_payload_z_7 ((Znth (i) (rows) ((@nil Z))))) )
+  **  (store_string substring_addr substring_l )
+  **  (PtrArray.seg data 0 output_size output_ptrs )
+  **  (PtrArray.undef_seg data output_size strings_size_pre )
+|--
+  “ (valid_string substring_l ) ” 
+  &&  “ ((string_length (substring_l)) < INT_MAX) ” 
+  &&  “ ((string_length ((row_payload_z_7 ((Znth (i) (rows) ((@nil Z))))))) < INT_MAX) ” 
+  &&  “ (valid_string (row_payload_z_7 ((Znth (i) (rows) ((@nil Z))))) ) ”
+) \/
+(
+forall (strings_size_pre: Z) (substring_addr: Z) (strings_addr: Z) (substring_l: (@list Z)) (rows: (@list (@list Z))) (row_ptr: Z) (output_rows: (@list (@list Z))) (output_ptrs: (@list Z)) (i: Z) (output_size: Z) (out: Z) (data: Z) (hit: Z) (PreH1 : (0 <= INT_MAX)) (PreH2 : (strings_size_pre <= INT_MAX)) (PreH3 : (output_size <= INT_MAX)) (PreH4 : (i <= INT_MAX)) (PreH5 : (0 >= INT_MIN)) (PreH6 : (strings_size_pre >= INT_MIN)) (PreH7 : (output_size >= INT_MIN)) (PreH8 : (i >= INT_MIN)) (PreH9 : (0 <= ((string_length (substring_l)) + 1 ))) (PreH10 : (0 <= ((string_length ((row_payload_z_7 ((Znth (i) (rows) ((@nil Z))))))) + 1 ))) (PreH11 : (0 <= i)) (PreH12 : (i < strings_size_pre)) (PreH13 : (0 <= output_size)) (PreH14 : (output_size <= i)) (PreH15 : (output_size = (Zlength (output_rows)))) (PreH16 : (output_size = (Zlength (output_ptrs)))) (PreH17 : (out <> 0)) (PreH18 : (data <> 0)) (PreH19 : (rows_well_formed_7 rows strings_size_pre )) (PreH20 : (row_well_formed_7 (Znth (i) (rows) ((@nil Z))) )) (PreH21 : (problem_7_pre_z rows )) (PreH22 : (valid_string substring_l )) (PreH23 : ((string_length (substring_l)) < INT_MAX)) (PreH24 : (filter_substring_state_7 rows substring_l i output_rows )) ,
+  (CharArray.full substring_addr ((string_length (substring_l)) + 1 ) (c_string (substring_l)) )
+  **  (CharArray.full row_ptr ((string_length ((row_payload_z_7 ((Znth (i) (rows) ((@nil Z))))))) + 1 ) (c_string ((row_payload_z_7 ((Znth (i) (rows) ((@nil Z))))))) )
+  **  ((( &( "i" ) )) # Int  |-> i)
+  **  ((( &( "output_size" ) )) # Int  |-> output_size)
+  **  ((( &( "strings" ) )) # Ptr  |-> strings_addr)
+  **  ((( &( "substring" ) )) # Ptr  |-> substring_addr)
+  **  ((( &( "strings_size" ) )) # Int  |-> strings_size_pre)
+  **  ((( &( "out" ) )) # Ptr  |-> out)
+  **  ((( &( "data" ) )) # Ptr  |-> data)
+  **  ((( &( "cur" ) )) # Ptr  |-> row_ptr)
+  **  ((( &( "hit" ) )) # Ptr  |-> hit)
+  **  ((&((out)  # "<anonymous struct>" ->ₛ "data")) # Ptr  |-> data)
+  **  ((&((out)  # "<anonymous struct>" ->ₛ "size")) # Int  |-> 0)
+  **  (CharPtrArray2.missing_i strings_addr strings_size_pre i row_ptr rows )
+  **  (((strings_addr + (i * sizeof(PTR) ) )) # Ptr  |-> row_ptr)
+  **  (PtrArray.seg data 0 output_size output_ptrs )
+  **  (PtrArray.undef_seg data output_size strings_size_pre )
+|--
+  “ (valid_string (row_payload_z_7 ((Znth (i) (rows) ((@nil Z))))) ) ” 
+  &&  “ ((string_length ((row_payload_z_7 ((Znth (i) (rows) ((@nil Z))))))) < INT_MAX) ”
+).
+
+Definition filter_by_substring_partial_solve_wit_3_pure_split_goal_1 := 
+forall (strings_size_pre: Z) (substring_addr: Z) (strings_addr: Z) (substring_l: (@list Z)) (rows: (@list (@list Z))) (row_ptr: Z) (output_rows: (@list (@list Z))) (output_ptrs: (@list Z)) (i: Z) (output_size: Z) (out: Z) (data: Z) (hit: Z) (PreH1 : (0 <= INT_MAX)) (PreH2 : (strings_size_pre <= INT_MAX)) (PreH3 : (output_size <= INT_MAX)) (PreH4 : (i <= INT_MAX)) (PreH5 : (0 >= INT_MIN)) (PreH6 : (strings_size_pre >= INT_MIN)) (PreH7 : (output_size >= INT_MIN)) (PreH8 : (i >= INT_MIN)) (PreH9 : (0 <= ((string_length (substring_l)) + 1 ))) (PreH10 : (0 <= ((string_length ((row_payload_z_7 ((Znth (i) (rows) ((@nil Z))))))) + 1 ))) (PreH11 : (0 <= i)) (PreH12 : (i < strings_size_pre)) (PreH13 : (0 <= output_size)) (PreH14 : (output_size <= i)) (PreH15 : (output_size = (Zlength (output_rows)))) (PreH16 : (output_size = (Zlength (output_ptrs)))) (PreH17 : (out <> 0)) (PreH18 : (data <> 0)) (PreH19 : (rows_well_formed_7 rows strings_size_pre )) (PreH20 : (row_well_formed_7 (Znth (i) (rows) ((@nil Z))) )) (PreH21 : (problem_7_pre_z rows )) (PreH22 : (valid_string substring_l )) (PreH23 : ((string_length (substring_l)) < INT_MAX)) (PreH24 : (filter_substring_state_7 rows substring_l i output_rows )) ,
+  (CharArray.full substring_addr ((string_length (substring_l)) + 1 ) (c_string (substring_l)) )
+  **  (CharArray.full row_ptr ((string_length ((row_payload_z_7 ((Znth (i) (rows) ((@nil Z))))))) + 1 ) (c_string ((row_payload_z_7 ((Znth (i) (rows) ((@nil Z))))))) )
+  **  ((( &( "i" ) )) # Int  |-> i)
+  **  ((( &( "output_size" ) )) # Int  |-> output_size)
+  **  ((( &( "strings" ) )) # Ptr  |-> strings_addr)
+  **  ((( &( "substring" ) )) # Ptr  |-> substring_addr)
+  **  ((( &( "strings_size" ) )) # Int  |-> strings_size_pre)
+  **  ((( &( "out" ) )) # Ptr  |-> out)
+  **  ((( &( "data" ) )) # Ptr  |-> data)
+  **  ((( &( "cur" ) )) # Ptr  |-> row_ptr)
+  **  ((( &( "hit" ) )) # Ptr  |-> hit)
+  **  ((&((out)  # "<anonymous struct>" ->ₛ "data")) # Ptr  |-> data)
+  **  ((&((out)  # "<anonymous struct>" ->ₛ "size")) # Int  |-> 0)
+  **  (CharPtrArray2.missing_i strings_addr strings_size_pre i row_ptr rows )
+  **  (((strings_addr + (i * sizeof(PTR) ) )) # Ptr  |-> row_ptr)
+  **  (PtrArray.seg data 0 output_size output_ptrs )
+  **  (PtrArray.undef_seg data output_size strings_size_pre )
+|--
+  “ (valid_string (row_payload_z_7 ((Znth (i) (rows) ((@nil Z))))) ) ”
+.
+
+Definition filter_by_substring_partial_solve_wit_3_pure_split_goal_2 := 
+forall (strings_size_pre: Z) (substring_addr: Z) (strings_addr: Z) (substring_l: (@list Z)) (rows: (@list (@list Z))) (row_ptr: Z) (output_rows: (@list (@list Z))) (output_ptrs: (@list Z)) (i: Z) (output_size: Z) (out: Z) (data: Z) (hit: Z) (PreH1 : (0 <= INT_MAX)) (PreH2 : (strings_size_pre <= INT_MAX)) (PreH3 : (output_size <= INT_MAX)) (PreH4 : (i <= INT_MAX)) (PreH5 : (0 >= INT_MIN)) (PreH6 : (strings_size_pre >= INT_MIN)) (PreH7 : (output_size >= INT_MIN)) (PreH8 : (i >= INT_MIN)) (PreH9 : (0 <= ((string_length (substring_l)) + 1 ))) (PreH10 : (0 <= ((string_length ((row_payload_z_7 ((Znth (i) (rows) ((@nil Z))))))) + 1 ))) (PreH11 : (0 <= i)) (PreH12 : (i < strings_size_pre)) (PreH13 : (0 <= output_size)) (PreH14 : (output_size <= i)) (PreH15 : (output_size = (Zlength (output_rows)))) (PreH16 : (output_size = (Zlength (output_ptrs)))) (PreH17 : (out <> 0)) (PreH18 : (data <> 0)) (PreH19 : (rows_well_formed_7 rows strings_size_pre )) (PreH20 : (row_well_formed_7 (Znth (i) (rows) ((@nil Z))) )) (PreH21 : (problem_7_pre_z rows )) (PreH22 : (valid_string substring_l )) (PreH23 : ((string_length (substring_l)) < INT_MAX)) (PreH24 : (filter_substring_state_7 rows substring_l i output_rows )) ,
+  (CharArray.full substring_addr ((string_length (substring_l)) + 1 ) (c_string (substring_l)) )
+  **  (CharArray.full row_ptr ((string_length ((row_payload_z_7 ((Znth (i) (rows) ((@nil Z))))))) + 1 ) (c_string ((row_payload_z_7 ((Znth (i) (rows) ((@nil Z))))))) )
+  **  ((( &( "i" ) )) # Int  |-> i)
+  **  ((( &( "output_size" ) )) # Int  |-> output_size)
+  **  ((( &( "strings" ) )) # Ptr  |-> strings_addr)
+  **  ((( &( "substring" ) )) # Ptr  |-> substring_addr)
+  **  ((( &( "strings_size" ) )) # Int  |-> strings_size_pre)
+  **  ((( &( "out" ) )) # Ptr  |-> out)
+  **  ((( &( "data" ) )) # Ptr  |-> data)
+  **  ((( &( "cur" ) )) # Ptr  |-> row_ptr)
+  **  ((( &( "hit" ) )) # Ptr  |-> hit)
+  **  ((&((out)  # "<anonymous struct>" ->ₛ "data")) # Ptr  |-> data)
+  **  ((&((out)  # "<anonymous struct>" ->ₛ "size")) # Int  |-> 0)
+  **  (CharPtrArray2.missing_i strings_addr strings_size_pre i row_ptr rows )
+  **  (((strings_addr + (i * sizeof(PTR) ) )) # Ptr  |-> row_ptr)
+  **  (PtrArray.seg data 0 output_size output_ptrs )
+  **  (PtrArray.undef_seg data output_size strings_size_pre )
+|--
+  “ ((string_length ((row_payload_z_7 ((Znth (i) (rows) ((@nil Z))))))) < INT_MAX) ”
+.
+
+Definition filter_by_substring_partial_solve_wit_3_aux := 
+forall (strings_size_pre: Z) (substring_addr: Z) (strings_addr: Z) (substring_l: (@list Z)) (rows: (@list (@list Z))) (row_ptr: Z) (output_rows: (@list (@list Z))) (output_ptrs: (@list Z)) (i: Z) (output_size: Z) (out: Z) (data: Z) (PreH1 : (0 <= i)) (PreH2 : (i < strings_size_pre)) (PreH3 : (0 <= output_size)) (PreH4 : (output_size <= i)) (PreH5 : (output_size = (Zlength (output_rows)))) (PreH6 : (output_size = (Zlength (output_ptrs)))) (PreH7 : (out <> 0)) (PreH8 : (data <> 0)) (PreH9 : (rows_well_formed_7 rows strings_size_pre )) (PreH10 : (row_well_formed_7 (Znth (i) (rows) ((@nil Z))) )) (PreH11 : (problem_7_pre_z rows )) (PreH12 : (valid_string substring_l )) (PreH13 : ((string_length (substring_l)) < INT_MAX)) (PreH14 : (filter_substring_state_7 rows substring_l i output_rows )) ,
+  ((&((out)  # "<anonymous struct>" ->ₛ "data")) # Ptr  |-> data)
+  **  ((&((out)  # "<anonymous struct>" ->ₛ "size")) # Int  |-> 0)
+  **  (CharPtrArray2.missing_i strings_addr strings_size_pre i row_ptr rows )
+  **  (((strings_addr + (i * sizeof(PTR) ) )) # Ptr  |-> row_ptr)
+  **  (store_string row_ptr (row_payload_z_7 ((Znth (i) (rows) ((@nil Z))))) )
+  **  (store_string substring_addr substring_l )
+  **  (PtrArray.seg data 0 output_size output_ptrs )
+  **  (PtrArray.undef_seg data output_size strings_size_pre )
+|--
+  “ (valid_string substring_l ) ” 
+  &&  “ ((string_length (substring_l)) < INT_MAX) ” 
+  &&  “ ((string_length ((row_payload_z_7 ((Znth (i) (rows) ((@nil Z))))))) < INT_MAX) ” 
+  &&  “ (valid_string (row_payload_z_7 ((Znth (i) (rows) ((@nil Z))))) ) ” 
+  &&  “ (0 <= ((string_length (substring_l)) + 1 )) ” 
+  &&  “ (0 <= ((string_length ((row_payload_z_7 ((Znth (i) (rows) ((@nil Z))))))) + 1 )) ” 
+  &&  “ (0 <= i) ” 
+  &&  “ (i < strings_size_pre) ” 
+  &&  “ (0 <= output_size) ” 
+  &&  “ (output_size <= i) ” 
+  &&  “ (output_size = (Zlength (output_rows))) ” 
+  &&  “ (output_size = (Zlength (output_ptrs))) ” 
+  &&  “ (out <> 0) ” 
+  &&  “ (data <> 0) ” 
+  &&  “ (rows_well_formed_7 rows strings_size_pre ) ” 
+  &&  “ (row_well_formed_7 (Znth (i) (rows) ((@nil Z))) ) ” 
+  &&  “ (problem_7_pre_z rows ) ” 
+  &&  “ (valid_string substring_l ) ” 
+  &&  “ ((string_length (substring_l)) < INT_MAX) ” 
+  &&  “ (filter_substring_state_7 rows substring_l i output_rows ) ”
+  &&  (store_string row_ptr (row_payload_z_7 ((Znth (i) (rows) ((@nil Z))))) )
+  **  (store_string substring_addr substring_l )
+  **  ((&((out)  # "<anonymous struct>" ->ₛ "data")) # Ptr  |-> data)
+  **  ((&((out)  # "<anonymous struct>" ->ₛ "size")) # Int  |-> 0)
+  **  (CharPtrArray2.missing_i strings_addr strings_size_pre i row_ptr rows )
+  **  (((strings_addr + (i * sizeof(PTR) ) )) # Ptr  |-> row_ptr)
+  **  (PtrArray.seg data 0 output_size output_ptrs )
+  **  (PtrArray.undef_seg data output_size strings_size_pre )
+.
+
+Definition filter_by_substring_partial_solve_wit_3 := filter_by_substring_partial_solve_wit_3_pure -> filter_by_substring_partial_solve_wit_3_aux.
+
+Definition filter_by_substring_partial_solve_wit_4 := 
+forall (strings_size_pre: Z) (substring_addr: Z) (strings_addr: Z) (substring_l: (@list Z)) (rows: (@list (@list Z))) (row_ptr: Z) (output_rows: (@list (@list Z))) (output_ptrs: (@list Z)) (i: Z) (output_size: Z) (hit: Z) (out: Z) (data: Z) (PreH1 : (0 <= i)) (PreH2 : (i < strings_size_pre)) (PreH3 : (0 <= output_size)) (PreH4 : (output_size <= i)) (PreH5 : (output_size = (Zlength (output_rows)))) (PreH6 : (output_size = (Zlength (output_ptrs)))) (PreH7 : (hit <> 0)) (PreH8 : (out <> 0)) (PreH9 : (data <> 0)) (PreH10 : (rows_well_formed_7 rows strings_size_pre )) (PreH11 : (problem_7_pre_z rows )) (PreH12 : (valid_string substring_l )) (PreH13 : ((string_length (substring_l)) < INT_MAX)) (PreH14 : (filter_substring_state_7 rows substring_l i output_rows )) (PreH15 : (substring_hit_z_7 (row_payload_z_7 ((Znth (i) (rows) ((@nil Z))))) substring_l )) ,
+  ((&((out)  # "<anonymous struct>" ->ₛ "data")) # Ptr  |-> data)
+  **  ((&((out)  # "<anonymous struct>" ->ₛ "size")) # Int  |-> 0)
+  **  (CharPtrArray2.missing_i strings_addr strings_size_pre i row_ptr rows )
+  **  (((strings_addr + (i * sizeof(PTR) ) )) # Ptr  |-> row_ptr)
+  **  (store_string row_ptr (row_payload_z_7 ((Znth (i) (rows) ((@nil Z))))) )
+  **  (store_string substring_addr substring_l )
+  **  (PtrArray.seg data 0 output_size output_ptrs )
+  **  (PtrArray.undef_seg data output_size strings_size_pre )
+|--
+  “ (0 <= ((string_length (substring_l)) + 1 )) ” 
+  &&  “ (0 <= ((string_length ((row_payload_z_7 ((Znth (i) (rows) ((@nil Z))))))) + 1 )) ” 
+  &&  “ (0 <= i) ” 
+  &&  “ (i < strings_size_pre) ” 
+  &&  “ (0 <= output_size) ” 
+  &&  “ (output_size <= i) ” 
+  &&  “ (output_size = (Zlength (output_rows))) ” 
+  &&  “ (output_size = (Zlength (output_ptrs))) ” 
+  &&  “ (hit <> 0) ” 
+  &&  “ (out <> 0) ” 
+  &&  “ (data <> 0) ” 
+  &&  “ (rows_well_formed_7 rows strings_size_pre ) ” 
+  &&  “ (problem_7_pre_z rows ) ” 
+  &&  “ (valid_string substring_l ) ” 
+  &&  “ ((string_length (substring_l)) < INT_MAX) ” 
+  &&  “ (filter_substring_state_7 rows substring_l i output_rows ) ” 
+  &&  “ (substring_hit_z_7 (row_payload_z_7 ((Znth (i) (rows) ((@nil Z))))) substring_l ) ”
+  &&  (((data + (output_size * sizeof(PTR) ) )) # Ptr  |->_)
+  **  (PtrArray.undef_seg data (output_size + 1 ) strings_size_pre )
+  **  (CharArray.full substring_addr ((string_length (substring_l)) + 1 ) (c_string (substring_l)) )
+  **  (CharArray.full row_ptr ((string_length ((row_payload_z_7 ((Znth (i) (rows) ((@nil Z))))))) + 1 ) (c_string ((row_payload_z_7 ((Znth (i) (rows) ((@nil Z))))))) )
+  **  ((&((out)  # "<anonymous struct>" ->ₛ "data")) # Ptr  |-> data)
+  **  ((&((out)  # "<anonymous struct>" ->ₛ "size")) # Int  |-> 0)
+  **  (CharPtrArray2.missing_i strings_addr strings_size_pre i row_ptr rows )
+  **  (((strings_addr + (i * sizeof(PTR) ) )) # Ptr  |-> row_ptr)
+  **  (PtrArray.seg data 0 output_size output_ptrs )
+.
+
+Module Type VC_Correct.
+
+Include ptr_array2_Strategy_Correct.
+Include char_array_Strategy_Correct.
+Include string_Strategy_Correct.
+
+Axiom proof_of_filter_by_substring_safety_wit_1 : filter_by_substring_safety_wit_1.
+Axiom proof_of_filter_by_substring_safety_wit_2 : filter_by_substring_safety_wit_2.
+Axiom proof_of_filter_by_substring_safety_wit_3 : filter_by_substring_safety_wit_3.
+Axiom proof_of_filter_by_substring_safety_wit_4 : filter_by_substring_safety_wit_4.
+Axiom proof_of_filter_by_substring_safety_wit_5 : filter_by_substring_safety_wit_5.
+Axiom proof_of_filter_by_substring_safety_wit_6 : filter_by_substring_safety_wit_6.
+Axiom proof_of_filter_by_substring_safety_wit_7 : filter_by_substring_safety_wit_7.
+Axiom proof_of_filter_by_substring_safety_wit_8 : filter_by_substring_safety_wit_8.
+Axiom proof_of_filter_by_substring_safety_wit_9 : filter_by_substring_safety_wit_9.
+Axiom proof_of_filter_by_substring_safety_wit_10 : filter_by_substring_safety_wit_10.
+Axiom proof_of_filter_by_substring_entail_wit_1 : filter_by_substring_entail_wit_1.
+Axiom proof_of_filter_by_substring_entail_wit_2 : filter_by_substring_entail_wit_2.
+Axiom proof_of_filter_by_substring_entail_wit_3 : filter_by_substring_entail_wit_3.
+Axiom proof_of_filter_by_substring_entail_wit_4 : filter_by_substring_entail_wit_4.
+Axiom proof_of_filter_by_substring_entail_wit_5 : filter_by_substring_entail_wit_5.
+Axiom proof_of_filter_by_substring_entail_wit_6 : filter_by_substring_entail_wit_6.
+Axiom proof_of_filter_by_substring_entail_wit_7_1 : filter_by_substring_entail_wit_7_1.
+Axiom proof_of_filter_by_substring_entail_wit_7_2 : filter_by_substring_entail_wit_7_2.
+Axiom proof_of_filter_by_substring_entail_wit_8 : filter_by_substring_entail_wit_8.
+Axiom proof_of_filter_by_substring_return_wit_1 : filter_by_substring_return_wit_1.
+Axiom proof_of_filter_by_substring_partial_solve_wit_1 : filter_by_substring_partial_solve_wit_1.
+Axiom proof_of_filter_by_substring_partial_solve_wit_2_pure : filter_by_substring_partial_solve_wit_2_pure.
+Axiom proof_of_filter_by_substring_partial_solve_wit_2 : filter_by_substring_partial_solve_wit_2.
+Axiom proof_of_filter_by_substring_partial_solve_wit_3_pure : filter_by_substring_partial_solve_wit_3_pure.
+Axiom proof_of_filter_by_substring_partial_solve_wit_3 : filter_by_substring_partial_solve_wit_3.
+Axiom proof_of_filter_by_substring_partial_solve_wit_4 : filter_by_substring_partial_solve_wit_4.
+
+End VC_Correct.
