QCP_examples/humaneval/spec_logic_rewrite_c_files/C_7_goal_check.v
@@ -1,0 +1,9 @@
+From SimpleC.EE Require Import C_7_goal C_7_proof_auto C_7_proof_manual.
+
+Module VC_Correctness : VC_Correct.
+  Include ptr_array2_strategy_proof.
+  Include char_array_strategy_proof.
+  Include string_strategy_proof.
+  Include C_7_proof_auto.
+  Include C_7_proof_manual.
+End VC_Correctness.
