QCP_examples/humaneval/spec_logic_rewrite_c_files/coins_7.v
@@ -1,0 +1,360 @@
+Require Import Coq.ZArith.ZArith.
+Require Import Coq.Lists.List.
+Require Import Coq.Strings.String.
+Require Import Coq.Strings.Ascii.
+Require Import Coq.micromega.Lia.
+From AUXLib Require Import ListLib.
+From SimpleC.StdLib Require Import string_lib.
+From SimpleC.SL Require Import IntLib.
+Import ListNotations.
+
+Load "../spec/7".
+Load "../StringClaude/string_bridge".
+
+Local Open Scope Z_scope.
+Local Open Scope string_scope.
+Local Open Scope list_scope.
+
+Definition row_payload_z_7 (row : list Z) : list Z :=
+  removelast row.
+
+Definition row_well_formed_7 (row : list Z) : Prop :=
+  row = c_string (row_payload_z_7 row) /\
+  valid_string (row_payload_z_7 row) /\
+  string_length (row_payload_z_7 row) < INT_MAX.
+
+Definition rows_well_formed_7 (rows : list (list Z)) (n : Z) : Prop :=
+  Zlength rows = n /\ Forall row_well_formed_7 rows.
+
+Definition rows_to_strings_z_7 (rows : list (list Z)) : list string :=
+  map (fun row => string_of_list_z (row_payload_z_7 row)) rows.
+
+Definition problem_7_pre_z (rows : list (list Z)) : Prop :=
+  problem_7_pre.
+
+Definition problem_7_spec_z
+    (rows : list (list Z)) (substring : list Z)
+    (output : list (list Z)) : Prop :=
+  problem_7_spec
+    (rows_to_strings_z_7 rows)
+    (map string_of_list_z output)
+    (string_of_list_z substring).
+
+Definition substring_hit_z_7 (str sub : list Z) : Prop :=
+  exists i, substring_at str sub i.
+
+Definition substring_miss_z_7 (str sub : list Z) : Prop :=
+  ~ substring_hit_z_7 str sub.
+
+Inductive filter_by_substring_z_7
+    : list (list Z) -> list Z -> list (list Z) -> Prop :=
+| fbsz_nil : forall sub,
+    filter_by_substring_z_7 [] sub []
+| fbsz_keep : forall h t sub output,
+    substring_hit_z_7 h sub ->
+    filter_by_substring_z_7 t sub output ->
+    filter_by_substring_z_7 (h :: t) sub (h :: output)
+| fbsz_drop : forall h t sub output,
+    ~ substring_hit_z_7 h sub ->
+    filter_by_substring_z_7 t sub output ->
+    filter_by_substring_z_7 (h :: t) sub output.
+
+Definition filter_substring_state_7
+    (rows : list (list Z)) (sub : list Z) (i : Z)
+    (output : list (list Z)) : Prop :=
+  filter_by_substring_z_7
+    (map row_payload_z_7 (sublist 0 i rows)) sub output.
+
+Lemma removelast_app_single_7 : forall {A : Type} (l : list A) x,
+  removelast (l ++ [x]) = l.
+Proof.
+  intros A l x. induction l as [|a l IH]; simpl; auto.
+  destruct l; simpl in *; congruence.
+Qed.
+
+Lemma row_payload_c_string_7 : forall payload,
+  row_payload_z_7 (c_string payload) = payload.
+Proof.
+  intros payload. unfold row_payload_z_7, c_string.
+  apply removelast_app_single_7.
+Qed.
+
+Lemma c_string_Zlength_7 : forall payload,
+  Zlength (c_string payload) = string_length payload + 1.
+Proof.
+  intros payload. unfold c_string, string_length.
+  rewrite Zlength_app, Zlength_cons, Zlength_nil. lia.
+Qed.
+
+Lemma rows_well_formed_length_7 : forall rows n,
+  rows_well_formed_7 rows n -> Zlength rows = n.
+Proof. intros rows n [H _]; exact H. Qed.
+
+Lemma rows_well_formed_nth_7 : forall rows n i,
+  rows_well_formed_7 rows n ->
+  0 <= i < n ->
+  row_well_formed_7 (Znth i rows []).
+Proof.
+  intros rows n i [Hlen Hall] Hi.
+  rewrite Forall_forall in Hall. apply Hall.
+  unfold Znth. apply nth_In.
+  apply Nat2Z.inj_lt. rewrite Z2Nat.id by lia.
+  rewrite <- Zlength_correct. lia.
+Qed.
+
+Lemma string_of_list_z_app_7 : forall a b,
+  string_of_list_z (a ++ b) =
+  (string_of_list_z a ++ string_of_list_z b)%string.
+Proof.
+  induction a as [|x a IH]; intros b; simpl; auto.
+  rewrite IH. reflexivity.
+Qed.
+
+Lemma substring_at_decompose_7 : forall str sub i,
+  substring_at str sub i ->
+  exists pre suf, str = pre ++ sub ++ suf.
+Proof.
+  intros str sub i [Hi [Hend Hpoint]].
+  unfold string_length in Hi, Hend, Hpoint.
+  pose proof (Zlength_nonneg sub) as Hsub_len.
+  exists (sublist 0 i str), (sublist (i + Zlength sub) (Zlength str) str).
+  assert (Hmid : sublist i (i + Zlength sub) str = sub).
+  {
+    apply (proj2 (list_eq_ext (sublist i (i + Zlength sub) str) sub 0)).
+    split.
+    - rewrite Zlength_sublist.
+      + lia.
+      + split.
+        * split; [exact (proj1 Hi) | lia].
+        * exact Hend.
+    - intros k Hk.
+      assert (Hk' : 0 <= k < Zlength sub).
+      { pose proof (Zlength_sublist i (i + Zlength sub) str) as Hlenmid.
+        specialize (Hlenmid ltac:(split; [split; [exact (proj1 Hi) | lia] | exact Hend])).
+        rewrite Hlenmid in Hk. lia. }
+      rewrite Znth_sublist.
+      2: exact (proj1 Hi).
+      2: lia.
+      replace (k + i) with (i + k) by lia.
+      apply Hpoint. exact Hk'.
+  }
+  assert (Hself : sublist 0 (Zlength str) str = str).
+  { apply sublist_self. reflexivity. }
+  rewrite <- Hself at 1.
+  rewrite (sublist_split 0 (Zlength str) i str).
+  2: { split; lia. }
+  2: { split; lia. }
+  rewrite (sublist_split i (Zlength str) (i + Zlength sub) str).
+  2: { split; lia. }
+  2: { split; lia. }
+  rewrite Hmid.
+  rewrite app_assoc.
+  reflexivity.
+Qed.
+
+Lemma decompose_substring_at_7 : forall str sub pre suf,
+  str = pre ++ sub ++ suf ->
+  substring_at str sub (Zlength pre).
+Proof.
+  intros str sub pre suf ->.
+  unfold substring_at, string_length.
+  pose proof (Zlength_nonneg pre).
+  pose proof (Zlength_nonneg sub).
+  pose proof (Zlength_nonneg suf).
+  repeat split.
+  - lia.
+  - rewrite !Zlength_app. lia.
+  - rewrite !Zlength_app. lia.
+  - intros k Hk.
+    rewrite app_Znth2 by lia.
+    replace (Zlength pre + k - Zlength pre) with k by lia.
+    rewrite app_Znth1 by exact Hk.
+    reflexivity.
+Qed.
+
+Definition z_of_ascii_7 (c : ascii) : Z :=
+  Z.of_nat (nat_of_ascii c).
+
+Lemma list_ascii_of_string_app_7 : forall a b,
+  list_ascii_of_string (a ++ b) =
+  (list_ascii_of_string a ++ list_ascii_of_string b)%list.
+Proof.
+  induction a; intros b; simpl; auto.
+  rewrite IHa. reflexivity.
+Qed.
+
+Lemma map_z_ascii_inverse_7 : forall l,
+  all_ascii l ->
+  map z_of_ascii_7 (map ascii_of_z l) = l.
+Proof.
+  induction l as [|x l IH]; intros Hall; simpl; auto.
+  f_equal.
+  - unfold z_of_ascii_7.
+    assert (Hx : 0 <= x < 256).
+    { specialize (Hall 0). rewrite Znth0_cons in Hall.
+      specialize (Hall ltac:(rewrite Zlength_cons; pose proof (Zlength_nonneg l); lia)).
+      lia. }
+    rewrite nat_of_ascii_ascii_of_z by exact Hx.
+    rewrite Z2Nat.id by lia. reflexivity.
+  - apply IH. intros i Hi.
+    specialize (Hall (i + 1)).
+    rewrite Znth_cons in Hall by lia.
+    replace (i + 1 - 1) with i in Hall by lia.
+    apply Hall. rewrite Zlength_cons. lia.
+Qed.
+
+Lemma substring_hit_string_7 : forall str sub,
+  all_ascii str ->
+  all_ascii sub ->
+  substring_hit_z_7 str sub <->
+  contains_substring (string_of_list_z str) (string_of_list_z sub).
+Proof.
+  intros str sub Hstr Hsub. split.
+  - intros [i Hi].
+    destruct (substring_at_decompose_7 str sub i Hi) as [pre [suf ->]].
+    exists (string_of_list_z pre), (string_of_list_z suf).
+    rewrite !string_of_list_z_app_7. reflexivity.
+  - intros [pre [suf H]].
+    apply (f_equal list_ascii_of_string) in H.
+    rewrite list_ascii_of_string_string_of_list_z in H.
+    rewrite !list_ascii_of_string_app_7 in H.
+    rewrite list_ascii_of_string_string_of_list_z in H.
+    apply (f_equal (map z_of_ascii_7)) in H.
+    rewrite !map_app in H.
+    rewrite (map_z_ascii_inverse_7 str Hstr) in H.
+    rewrite (map_z_ascii_inverse_7 sub Hsub) in H.
+    exists (Zlength (map z_of_ascii_7 (list_ascii_of_string pre))).
+    apply decompose_substring_at_7 with
+      (pre := map z_of_ascii_7 (list_ascii_of_string pre))
+      (suf := map z_of_ascii_7 (list_ascii_of_string suf)).
+    exact H.
+Qed.
+
+Lemma filter_substring_state_nil_7 : forall rows sub,
+  filter_substring_state_7 rows sub 0 [].
+Proof.
+  intros rows sub. unfold filter_substring_state_7.
+  simpl [sublist]. constructor.
+Qed.
+
+Lemma filter_by_substring_z_snoc_keep_7 : forall input sub output h,
+  filter_by_substring_z_7 input sub output ->
+  substring_hit_z_7 h sub ->
+  filter_by_substring_z_7 (input ++ [h]) sub (output ++ [h]).
+Proof.
+  intros input sub output h Hfilter Hhit.
+  induction Hfilter; simpl.
+  - constructor; [exact Hhit | constructor].
+  - constructor; auto.
+  - apply fbsz_drop; auto.
+Qed.
+
+Lemma filter_by_substring_z_snoc_drop_7 : forall input sub output h,
+  filter_by_substring_z_7 input sub output ->
+  ~ substring_hit_z_7 h sub ->
+  filter_by_substring_z_7 (input ++ [h]) sub output.
+Proof.
+  intros input sub output h Hfilter Hmiss.
+  induction Hfilter; simpl.
+  - apply fbsz_drop; [exact Hmiss | constructor].
+  - constructor; auto.
+  - apply fbsz_drop; auto.
+Qed.
+
+Lemma filter_substring_state_keep_7 : forall rows sub i output,
+  0 <= i < Zlength rows ->
+  filter_substring_state_7 rows sub i output ->
+  substring_hit_z_7 (row_payload_z_7 (Znth i rows [])) sub ->
+  filter_substring_state_7 rows sub (i + 1)
+    (output ++ [row_payload_z_7 (Znth i rows [])]).
+Proof.
+  intros rows sub i output Hi Hstate Hhit.
+  unfold filter_substring_state_7 in *.
+  rewrite (sublist_split 0 (i + 1) i rows) by lia.
+  rewrite (@sublist_single (list Z) [] i rows) by lia. simpl.
+  rewrite map_app. simpl.
+  apply filter_by_substring_z_snoc_keep_7; assumption.
+Qed.
+
+Lemma filter_substring_state_drop_7 : forall rows sub i output,
+  0 <= i < Zlength rows ->
+  filter_substring_state_7 rows sub i output ->
+  ~ substring_hit_z_7 (row_payload_z_7 (Znth i rows [])) sub ->
+  filter_substring_state_7 rows sub (i + 1) output.
+Proof.
+  intros rows sub i output Hi Hstate Hmiss.
+  unfold filter_substring_state_7 in *.
+  rewrite (sublist_split 0 (i + 1) i rows) by lia.
+  rewrite (@sublist_single (list Z) [] i rows) by lia. simpl.
+  rewrite map_app. simpl.
+  apply filter_by_substring_z_snoc_drop_7; assumption.
+Qed.
+
+Lemma strstr_result_hit_7 : forall str sub ret base,
+  strstr_result str sub ret base ->
+  ret <> 0 -> substring_hit_z_7 str sub.
+Proof.
+  intros str sub ret base [Hhit | [Hnone ->]] Hret.
+  - destruct Hhit as [i [Hi _]]. exists i. exact Hi.
+  - contradiction.
+Qed.
+
+Lemma strstr_result_miss_7 : forall str sub ret base,
+  strstr_result str sub ret base ->
+  ret = 0 -> ~ substring_hit_z_7 str sub.
+Proof.
+  intros str sub ret base [Hhit | [Hnone _]] Hzero [i Hi].
+  - destruct Hhit as [j [_ [_ [Hret Hnz]]]]. subst ret. contradiction.
+  - apply (Hnone i (proj1 Hi)). exact Hi.
+Qed.
+
+Lemma filter_by_substring_z_sound_7 : forall input sub output,
+  Forall all_ascii input ->
+  all_ascii sub ->
+  filter_by_substring_z_7 input sub output ->
+  filter_by_substring
+    (map string_of_list_z input)
+    (string_of_list_z sub)
+    (map string_of_list_z output).
+Proof.
+  intros input sub output Hinput Hsub Hfilter.
+  induction Hfilter; simpl in *.
+  - constructor.
+  - inversion Hinput; subst.
+    constructor.
+    + apply (proj1 (substring_hit_string_7 h sub H2 Hsub)); exact H.
+    + apply IHHfilter; assumption.
+  - apply fbsr_drop.
+    + inversion Hinput; subst.
+      intro Hcontains. apply H.
+      apply (proj2 (substring_hit_string_7 h sub H2 Hsub)); exact Hcontains.
+    + inversion Hinput; subst. apply IHHfilter; assumption.
+Qed.
+
+Lemma rows_well_formed_payload_ascii_7 : forall rows n,
+  rows_well_formed_7 rows n ->
+  Forall all_ascii (map row_payload_z_7 rows).
+Proof.
+  intros rows n [_ Hall].
+  induction Hall; simpl; constructor; auto.
+  unfold row_well_formed_7 in H.
+  destruct H as [_ [[Hascii _] _]]. exact Hascii.
+Qed.
+
+Lemma problem_7_spec_z_of_filter_state : forall rows sub output,
+  rows_well_formed_7 rows (Zlength rows) ->
+  valid_string sub ->
+  filter_substring_state_7 rows sub (Zlength rows) output ->
+  problem_7_spec_z rows sub output.
+Proof.
+  intros rows sub output Hrows [Hsub _] Hstate.
+  unfold filter_substring_state_7 in Hstate.
+  rewrite sublist_self in Hstate by reflexivity.
+  unfold problem_7_spec_z, problem_7_spec, rows_to_strings_z_7.
+  rewrite <- map_map.
+  apply filter_by_substring_z_sound_7.
+  - apply rows_well_formed_payload_ascii_7 with (n := Zlength rows).
+    exact Hrows.
+  - exact Hsub.
+  - exact Hstate.
+Qed.
